x86/Symbtablegenproof.v
@@ -1,0 +1,2047 @@
+(* *******************  *)
+(* Author: Yuting Wang  *)
+(* Date:   Dec 2, 2019 *)
+(* *******************  *)
+
+Require Import Coqlib Errors Maps.
+Require Import Integers Floats AST Linking.
+Require Import Values Memory Events Globalenvs Smallstep.
+Require Import Op Locations Mach Conventions Asm RealAsm.
+Require Import Symbtablegen.
+Require Import RelocProg RelocProgram RelocProgSemantics.
+Require Import LocalLib.
+Import ListNotations.
+Require AsmFacts.
+
+Open Scope Z_scope.
+
+Hint Resolve in_eq in_cons.
+
+Ltac monadInvX1 H :=
+  let monadInvX H :=  
+      monadInvX1 H ||
+                 match type of H with
+                 | (?F _ _ _ _ _ _ _ _ = OK _) =>
+                   ((progress simpl in H) || unfold F in H); monadInvX1 H
+                 | (?F _ _ _ _ _ _ _ = OK _) =>
+                   ((progress simpl in H) || unfold F in H); monadInvX1 H
+                 | (?F _ _ _ _ _ _ = OK _) =>
+                   ((progress simpl in H) || unfold F in H); monadInvX1 H
+                 | (?F _ _ _ _ _ = OK _) =>
+                   ((progress simpl in H) || unfold F in H); monadInvX1 H
+                 | (?F _ _ _ _ = OK _) =>
+                   ((progress simpl in H) || unfold F in H); monadInvX1 H
+                 | (?F _ _ _ = OK _) =>
+                   ((progress simpl in H) || unfold F in H); monadInvX1 H
+                 | (?F _ _ = OK _) =>
+                   ((progress simpl in H) || unfold F in H); monadInvX1 H
+                 | (?F _ = OK _) =>
+                   ((progress simpl in H) || unfold F in H); monadInvX1 H
+                 end
+  in
+
+  match type of H with
+  | (OK _ = OK _) =>
+      inversion H; clear H; try subst
+  | (Error _ = OK _) =>
+      discriminate
+  | (bind ?F ?G = OK ?X) =>
+      let x := fresh "x" in (
+      let EQ1 := fresh "EQ" in (
+      let EQ2 := fresh "EQ" in (
+      destruct (bind_inversion F G H) as [x [EQ1 EQ2]];
+      clear H;
+      try (monadInvX EQ1);
+      try (monadInvX1 EQ2))))
+  | (bind2 ?F ?G = OK ?X) =>
+      let x1 := fresh "x" in (
+      let x2 := fresh "x" in (
+      let EQ1 := fresh "EQ" in (
+      let EQ2 := fresh "EQ" in (
+      destruct (bind2_inversion F G H) as [x1 [x2 [EQ1 EQ2]]];
+      clear H;
+      try (monadInvX EQ1);
+      try (monadInvX1 EQ2)))))
+  | (match ?X with left _ => _ | right _ => assertion_failed end = OK _) =>
+      destruct X eqn:?; [try (monadInvX1 H) | discriminate]
+  | (match (negb ?X) with true => _ | false => assertion_failed end = OK _) =>
+      destruct X as [] eqn:?; [discriminate | try (monadInvX1 H)]
+  | (match ?X with true => _ | false => assertion_failed end = OK _) =>
+      destruct X as [] eqn:?; [try (monadInvX1 H) | discriminate]
+  | (mmap ?F ?L = OK ?M) =>
+      generalize (mmap_inversion F L H); intro
+  | (match ?X with Some _ => _ | None => _ end = _) =>
+      let EQ := fresh "EQ" in (
+      destruct X eqn:EQ; try (monadInvX1 H))
+  | (match ?X with pair _ _ => _ end = OK _) =>
+      let EQ := fresh "EQ" in (
+      destruct X eqn:EQ; try (monadInvX1 H))
+  end.
+
+Ltac monadInvX H :=
+  monadInvX1 H ||
+  match type of H with
+  | (?F _ _ _ _ _ _ _ _ = OK _) =>
+      ((progress simpl in H) || unfold F in H); monadInvX1 H
+  | (?F _ _ _ _ _ _ _ = OK _) =>
+      ((progress simpl in H) || unfold F in H); monadInvX1 H
+  | (?F _ _ _ _ _ _ = OK _) =>
+      ((progress simpl in H) || unfold F in H); monadInvX1 H
+  | (?F _ _ _ _ _ = OK _) =>
+      ((progress simpl in H) || unfold F in H); monadInvX1 H
+  | (?F _ _ _ _ = OK _) =>
+      ((progress simpl in H) || unfold F in H); monadInvX1 H
+  | (?F _ _ _ = OK _) =>
+      ((progress simpl in H) || unfold F in H); monadInvX1 H
+  | (?F _ _ = OK _) =>
+      ((progress simpl in H) || unfold F in H); monadInvX1 H
+  | (?F _ = OK _) =>
+      ((progress simpl in H) || unfold F in H); monadInvX1 H
+  end.  
+
+Lemma alignw_le : forall x, x <= align x alignw.
+Proof.
+  intros x. apply align_le. unfold alignw. lia.
+Qed.
+
+
+Lemma divides_align : forall y x,
+    y > 0 -> (y | x) -> align x y = x.
+Proof.
+  intros y x GT DV.
+  unfold align. red in DV. destruct DV as [z DV].
+  subst. replace (z * y + y - 1) with (z * y + (y - 1)) by lia.
+  erewrite Zbits.Zdiv_shift; eauto.
+  erewrite Z_div_mult; eauto. rewrite Z_mod_mult.
+  rewrite zeq_true. rewrite Z.add_0_r. auto.
+Qed.
+
+Lemma align_idempotent : forall v x,
+    x > 0 -> align (align v x) x = align v x.
+Proof.
+  intros v x H. eapply divides_align; eauto.
+  apply align_divides. auto.
+Qed.
+
+Lemma alignw_divides:
+  forall z,
+    (alignw | align z alignw).
+Proof.
+  intros. apply align_divides. unfold alignw; lia.
+Qed.
+
+(* Lemma fold_left_acc_symb_acc: *)
+(*   forall defs stbl rodofs dofs cofs stbl' rodofs' dofs' cofs', *)
+(*     fold_left (acc_symb sec_rodata_id sec_data_id sec_code_id) defs (stbl, rodofs, dofs, cofs) = (stbl', rodofs', dofs', cofs') -> *)
+(*     forall se, *)
+(*       In se stbl -> In se stbl'. *)
+(* Proof. *)
+(*   induction defs; simpl; intros; eauto. inv H; auto. *)
+(*   repeat destr_in H. *)
+(*   eapply IHdefs. eauto. right. auto. *)
+(* Qed. *)
+
+(* Lemma gen_symb_table_ok: *)
+(*   forall id d defs defs1 defs2 stbl rodofs dofs cofs stbl' rodofs' dofs' cofs', *)
+(*     defs = defs1 ++ (id, d) :: defs2 -> *)
+(*     list_norepet (map fst defs) -> *)
+(*     fold_left (acc_symb sec_rodata_id sec_data_id sec_code_id) defs (stbl, rodofs, dofs, cofs) = (stbl', rodofs', dofs', cofs') -> *)
+(*     exists rodofs1 dofs1 cofs1 stbl1, *)
+(*       fold_left (acc_symb sec_rodata_id sec_data_id sec_code_id) defs1 (stbl, rodofs, dofs, cofs) = (stbl1, rodofs1, dofs1, cofs1) /\ *)
+(*       In (get_symbentry sec_rodata_id sec_data_id sec_code_id rodofs1 dofs1 cofs1 id d) stbl'. *)
+(* Proof. *)
+(*   induction defs; simpl; intros defs1 defs2 stbl rodofs dofs cofs stbl' rodofs' dofs' cofs' SPLIT NR FL; eauto. *)
+(*   - apply (f_equal (@length _)) in SPLIT. *)
+(*     rewrite app_length in SPLIT. simpl in SPLIT. omega. *)
+(*   - repeat destr_in FL. *)
+(*     destruct (ident_eq i id). *)
+(*     + subst. *)
+(*       assert (defs1 = []). destruct defs1. auto. simpl in SPLIT. inv SPLIT. *)
+(*       simpl in NR. *)
+(*       inv NR. *)
+(*       exfalso; apply H2. rewrite map_app. rewrite in_app. right. simpl. auto. subst. *)
+(*       simpl in *. inv SPLIT. *)
+(*       (do 4 eexists); split; eauto. *)
+(*       eapply fold_left_acc_symb_acc. eauto. left; auto. *)
+(*     + destruct defs1. simpl in SPLIT. inv SPLIT. congruence. *)
+(*       simpl in SPLIT. inv SPLIT. *)
+(*       edestruct IHdefs as (rodofs1 & dofs1 & cofs1 & stbl1 & FL1 & IN1). eauto. *)
+(*       inv NR. auto. eauto. *)
+(*       simpl. rewrite Heqp0. *)
+(*       setoid_rewrite FL1. *)
+(*       (do 4 eexists); split; eauto. *)
+(* Qed. *)
+
+(* Lemma symb_table_ok: *)
+(*   forall id d defs rodofs dofs cofs stbl defs1 defs2, *)
+(*     defs = defs1 ++ (id, d) :: defs2 -> *)
+(*     list_norepet (map fst defs) -> *)
+(*     gen_symb_table sec_rodata_id sec_data_id sec_code_id defs = (stbl, rodofs, dofs, cofs) -> *)
+(*     exists stbl1 rodofs1 dofs1 cofs1, *)
+(*       gen_symb_table sec_rodata_id sec_data_id sec_code_id defs1 = (stbl1, rodofs1, dofs1, cofs1) /\ *)
+(*       In (get_symbentry sec_rodata_id sec_data_id sec_code_id rodofs1 dofs1 cofs1 id d) stbl. *)
+(* Proof. *)
+(*   intros. *)
+(*   unfold gen_symb_table in H1. repeat destr_in H1. *)
+(*   setoid_rewrite <- in_rev. *)
+(*   eapply gen_symb_table_ok in Heqp; eauto. *)
+(*   destruct Heqp as (rodofs1 & dofs1 & cofs1 & stbl1 & FL1 & IN1). *)
+(*   unfold gen_symb_table. setoid_rewrite FL1. *)
+(*   (do 4 eexists); split; eauto. *)
+(* Qed. *)
+
+(** Properties about Symbol Environments *)
+(* Lemma add_external_global_pres_senv : *)
+(*   forall e (ge : Genv.t) extfuns, *)
+(*   Genv.genv_senv (add_external_global extfuns ge e) = Genv.genv_senv ge. *)
+(* Proof. *)
+(*   intros. unfold add_external_global. *)
+(*   destr. *)
+(* Qed. *)
+
+(* Lemma add_external_globals_pres_senv : *)
+(*   forall stbl (ge : Genv.t) extfuns, *)
+(*   Genv.genv_senv (add_external_globals extfuns ge stbl) = Genv.genv_senv ge. *)
+(* Proof. *)
+(*   induction stbl; intros. *)
+(*   - simpl. auto. *)
+(*   - simpl. erewrite IHstbl; eauto. *)
+(* Qed. *)
+
+Lemma transf_prog_pres_senv: forall instr_size p tp,
+  transf_program instr_size p = OK tp -> 
+  Globalenvs.Genv.to_senv (Globalenvs.Genv.globalenv p) = Genv.genv_senv (globalenv instr_size tp).
+Proof.
+  intros instr_size p tp TF.
+  unfold transf_program in TF.
+  destr_in TF. destr_in TF. destr_in TF. (* destr_in TF. *)
+  (* destruct p. simpl. *)
+  (* destr_in TF. *)
+  (* inv TF. cbn. *)
+  (* rewrite add_external_globals_pres_senv. *)
+  cbn. auto.
+Qed.
+
+(** * Main Preservaiton Proofs *)
+Section PRESERVATION.
+
+Variable instr_size : instruction -> Z.
+  
+(** Assumption about external calls.
+    These should be merged into common properties about external calls later. *)
+Axiom external_call_inject : forall ge j vargs1 vargs2 m1 m2 m1' vres1 t ef,
+    Val.inject_list j vargs1 vargs2 ->
+    Mem.inject j m1 m2 ->
+    external_call ef ge vargs1 m1 t vres1 m1' ->
+    exists j' vres2 m2',
+      external_call ef ge vargs2 m2 t vres2 m2' /\
+      Val.inject j' vres1 vres2 /\ Mem.inject j' m1' m2' /\
+      inject_incr j j' /\
+      inject_separated j j' m1 m2.
+
+Axiom  external_call_valid_block: forall ef ge vargs m1 t vres m2 b,
+    external_call ef ge vargs m1 t vres m2 -> Mem.valid_block m1 b -> Mem.valid_block m2 b.
+
+
+Lemma prog_instr_valid: forall prog tprog,
+    transf_program instr_size prog = OK tprog ->
+    Forall def_instrs_valid (map snd (AST.prog_defs prog)).
+Proof.
+  intros prog tprog TRANSF.
+  unfold transf_program in TRANSF.
+  destr_in TRANSF.
+  inv w. auto.
+Qed.
+
+Lemma int_funct_instr_valid: forall prog tprog f b,
+    transf_program instr_size prog = OK tprog ->
+    Globalenvs.Genv.find_funct_ptr (Genv.globalenv prog) b = Some (Internal f) ->
+    Forall instr_valid (Asm.fn_code f).
+Proof.
+  intros prog tprog f b TF FIND.
+  generalize (prog_instr_valid _ _ TF).
+  intros NJ.
+  generalize (Genv.find_funct_ptr_inversion _ _ FIND).
+  intros (id, IN).
+  generalize (in_map snd _ _ IN).
+  cbn. intros IN'.
+  rewrite Forall_forall in NJ.
+  apply NJ in IN'.
+  red in IN'. auto.
+Qed.
+
+Lemma instr_is_valid: forall prog tprog f b i ofs,
+    transf_program instr_size prog = OK tprog ->
+    Globalenvs.Genv.find_funct_ptr (Genv.globalenv prog) b = Some (Internal f) ->
+    Asm.find_instr instr_size ofs (Asm.fn_code f) = Some i ->
+    instr_valid i.
+Proof.
+  intros prog tprog f b i ofs TF FIND FIND'.
+  generalize (int_funct_instr_valid _ _ _ _ TF FIND).
+  intros NJ.
+  rewrite Forall_forall in NJ.
+  auto. 
+  apply NJ. 
+  eapply Asmgenproof0.find_instr_in; eauto.
+Qed.
+  
+
+
+(** Transformation *)
+Variable prog: Asm.program.
+Variable tprog: program.
+
+Let ge := Genv.globalenv prog.
+Let tge := globalenv instr_size tprog.
+
+Definition match_prog (p: Asm.program) (tp: program) :=
+  transf_program instr_size p = OK tp.
+
+Hypothesis TRANSF: match_prog prog tprog.
+
+
+(** ** Definitions of Matching States *)
+
+Definition glob_block_valid (m:mem) := 
+  forall b g, Globalenvs.Genv.find_def ge b = Some g -> Mem.valid_block m b.
+
+(** Properties about the memory injection from RealAsm to Relocatable Programs *)   Record match_inj (j: meminj) : Type :=
+  {
+    (** Preservation of finding of instruction *)
+    agree_inj_instrs:
+      forall b b' f ofs ofs' i,
+        Globalenvs.Genv.find_funct_ptr ge b = Some (Internal f) ->
+        Asm.find_instr instr_size (Ptrofs.unsigned ofs) (Asm.fn_code f) = Some i ->
+        j b = Some (b', ofs') ->
+        Genv.find_instr tge (Vptr b' (Ptrofs.add ofs (Ptrofs.repr ofs'))) = Some i;
+
+    (** Preservation of finding of global symbols *)
+    agree_inj_globs:
+      forall id b,
+        Globalenvs.Genv.find_symbol ge id = Some b ->
+        exists b' ofs', Genv.find_symbol tge id = Some (b', ofs') /\
+                   j b = Some (b', Ptrofs.unsigned ofs');
+
+    (** Preservation of finding of external functions *)
+    agree_inj_ext_funct:
+      forall b f ofs b',
+        Globalenvs.Genv.find_funct_ptr ge b = Some (External f) ->
+        j b = Some (b', ofs) ->
+        Genv.find_ext_funct tge (Vptr b' (Ptrofs.repr ofs)) = Some f;
+
+    (** Preservation of finding of internal functions *)
+    agree_inj_int_funct:
+      forall b f ofs b' ofs',
+        Globalenvs.Genv.find_funct_ptr ge b = Some (Internal f) ->
+        j b = Some (b', ofs) ->
+        Genv.find_ext_funct tge (Vptr b' ofs') = None;
+  }.
+
+(** Match States *)
+(* Inductive match_states: state -> state -> Prop := *)
+(* | match_states_intro: forall (j:meminj) (rs: regset) (m: mem) (rs': regset) (m':mem) *)
+(*                         (MINJ: Mem.inject j (def_frame_inj m) m m') *)
+(*                         (MATCHINJ: match_inj j) *)
+(*                         (RSINJ: regset_inject j rs rs') *)
+(*                         (GBVALID: glob_block_valid m), *)
+(*     match_states (State rs m) (State rs' m'). *)
+
+Definition regset_inject (j: meminj) (rs1 rs2: regset) : Prop :=
+  forall r, Val.inject j (rs1#r) (rs2#r).
+
+Inductive match_states: state -> state -> Prop :=
+| match_states_intro: forall (rs: regset) (m: mem) (rs': regset) (m':mem) (j:meminj)
+                        (STRUCTJ: j = Mem.flat_inj (Mem.support m))
+                        (MATCHINJ: match_inj j)
+                        (MINJ: Mem.inject j  m m')
+                        (RSINJ: regset_inject j rs rs')
+                        (GBVALID: glob_block_valid m),
+    match_states (State rs m) (State rs' m').
+
+
+
+(** ** Matching of the Initial States *)
+  
+Lemma symbol_address_inject : forall j id ofs
+                                (MATCHINJ: match_inj j),
+    Val.inject j (Senv.symbol_address ge id ofs) (Genv.symbol_address tge id ofs).
+Proof.
+  intros. unfold Senv.symbol_address.
+  inv MATCHINJ.
+  unfold Senv.find_symbol. simpl.
+  destruct (Globalenvs.Genv.find_symbol ge id) eqn:FINDSYM; auto.
+  exploit agree_inj_globs0; eauto.
+  intros (b' & ofs' & FINDSYM' & JB).
+  erewrite Genv.symbol_address_offset; eauto. 
+  eapply Val.inject_ptr; eauto.
+  rewrite Ptrofs.repr_unsigned. apply Ptrofs.add_commut.
+  unfold Genv.symbol_address. rewrite FINDSYM'. 
+  rewrite Ptrofs.add_zero_l. auto.
+Qed.
+
+Section INIT_MEM.
+
+Variables m tm: mem.
+Hypothesis IM: Genv.init_mem prog = Some m.
+Hypothesis TIM: init_mem instr_size tprog = Some tm.
+
+
+(** Initial Memory Injection *)
+(* Definition init_meminj : meminj := *)
+(*   fun b => *)
+(*     (* (genv_next ge) is the stack block of the source program *) *)
+(*     match b with *)
+(*     | Stack _ _ _ => b *)
+(*     | Global id => *)
+(*     else *)
+(*       match (Globalenvs.Genv.invert_symbol ge b) with *)
+(*       | None => None *)
+(*       | Some id => *)
+(*         match Genv.find_symbol tge id with *)
+(*         | None => None *)
+(*         | Some (b,ofs) => Some (b, Ptrofs.unsigned ofs) *)
+(*         end *)
+(*       end. *)
+
+Theorem init_meminj_match_sminj :
+    match_inj (Mem.flat_inj (Mem.support m)).
+Proof.
+  constructor.
+  admit.
+  admit.
+  admit.
+  admit.
+Admitted.  
+(*   generalize TRANSF. intros TRANSF'. *)
+(*   unfold match_prog in TRANSF'. *)
+(*   unfold transf_program in TRANSF'. *)
+(*   repeat destr_in TRANSF'.  *)
+(*   destruct p. inv Heqp0. monadInv TRANSF'. *)
+(*   revert H0. intros TL. *)
+(*   constructor. *)
+
+(*   - (* agree_inj_instrs *) *)
+(*     intros b b' f ofs ofs' i FPTR FINST INITINJ. *)
+(*     unfold init_meminj in INITINJ.  *)
+(*     (* revert TL. *) *)
+(*     destruct eq_block. inv INITINJ. *)
+(*     unfold ge in FPTR. exploit Genv.genv_next_find_funct_ptr_absurd; eauto. contradiction. *)
+(*     destr_match_in INITINJ; inv INITINJ. *)
+(*     destr_match_in H0; inv H0. *)
+(*     destruct p. inv H1. rewrite Ptrofs.repr_unsigned. *)
+(*     unfold globalenv in EQ0; simpl in EQ0. *)
+(*     rewrite add_external_globals_pres_find_symbol in EQ0. *)
+(*     unfold Genv.find_symbol in EQ0. cbn in EQ0. *)
+(*     apply Genv.invert_find_symbol in EQ. *)
+(*     exploit (Genv.find_symbol_funct_ptr_inversion prog); eauto. *)
+(*     intros FINPROG. *)
+(*     unfold Genv.find_instr. unfold tge. *)
+(*     cbn. *)
+(*     rewrite add_external_globals_pres_instrs. cbn. *)
+(*     unfold create_sec_table. *)
+(*     replace (Pos.to_nat 1) with 1%nat by xomega. *)
+(*     cbn. *)
+(*     unfold gen_symb_table in Heqp. *)
+(*     destr_in Heqp. destruct p. destruct p. inv Heqp. *)
+(*     exploit acc_symb_tree_entry_some; eauto. *)
+(*     { inv w. auto. } *)
+(*     { eapply PTree_Properties.of_list_norepet; eauto. *)
+(*       inv w. auto. } *)
+(*     cbn. intros GET. *)
+(*     inversion w. *)
+(*     unfold gen_symb_map in EQ0. *)
+(*     exploit symbtable_to_tree_acc_symb_map_inv; eauto. *)
+(*     erewrite <- acc_symb_pres_ids; eauto.  *)
+(*     cbn. intros (EQOFS & i' & SEC & EQB). subst. *)
+(*     inv SEC. *)
+(*     eapply pres_find_instr; eauto.  *)
+(*     exploit Genv.find_symbol_funct_ptr_inversion; eauto. *)
+(*     apply Genv.invert_find_symbol. eauto. eauto. intros IN. *)
+(*     eapply gen_symb_table_only_internal_symbol; eauto. *)
+(*     inv w; auto. *)
+(*     cbn. auto. *)
+
+(*   - (* agree_inj_globs *) *)
+(*     intros id b FSYM. *)
+(*     unfold init_meminj. *)
+(*     destruct eq_block.  *)
+(*     subst b. exfalso. eapply Genv.find_symbol_genv_next_absurd; eauto. *)
+(*     exploit Genv.find_invert_symbol; eauto. intros INV. *)
+(*     unfold ge in INV. rewrite INV. *)
+(*     assert (exists b' ofs', Genv.find_symbol tge id = Some (b', ofs')) as FIND'. *)
+(*     {  *)
+(*       unfold ge in FSYM. *)
+(*       exploit Genv.find_symbol_inversion; eauto. intros INSYM. *)
+(*       unfold prog_defs_names in INSYM. *)
+(*       apply PTree_Properties.of_list_dom in INSYM. *)
+(*       destruct INSYM as (def & GET). *)
+(*       inversion w. *)
+(*       unfold gen_symb_table in Heqp. destr_in Heqp. *)
+(*       destruct p. destruct p. inv Heqp. *)
+(*       exploit acc_symb_tree_entry_some; eauto. *)
+(*       intros GET'. *)
+(*       unfold globalenv in tge; cbn in tge. *)
+(*       cbn in GET'. *)
+(*       unfold tge. *)
+(*       unfold symbtable_to_tree in GET'. *)
+(*       apply PTree_Properties.in_of_list in GET'. *)
+(*       set (e:= get_symbentry sec_rodata_id sec_data_id sec_code_id *)
+(*                              (defs_rodata_size (defs_before id (AST.prog_defs prog))) *)
+(*                              (defs_data_size (defs_before id (AST.prog_defs prog))) *)
+(*                              (defs_code_size (defs_before id (AST.prog_defs prog))) id def) in GET'. *)
+(*       destruct (is_def_internal is_fundef_internal def) eqn:INT. *)
+(*       * *)
+(*         assert (is_symbentry_internal e = true) as INT'. *)
+(*         { subst e. *)
+(*           erewrite <- get_symbentry_pres_internal_prop; eauto. } *)
+(*         assert (In e (rev s)) as IN'. *)
+(*         { unfold symbtable_to_idlist in GET'. *)
+(*           erewrite in_map_iff in GET'.  *)
+(*           destruct GET' as (e' & EQ & IN''). inversion EQ.  subst e'. auto. *)
+(*         }  *)
+(*         erewrite acc_symb_pres_ids in wf_prog_norepet_defs; eauto. *)
+(*         generalize (acc_symb_map_get_some_int _ _ (PTree.empty _) *)
+(*                                               wf_prog_norepet_defs IN' INT'). *)
+(*         intros (b' & ofs' & GET''). *)
+(*         assert (symbentry_id e = id) as IDEQ. *)
+(*         { subst e. rewrite get_symbentry_id. auto. } *)
+        
+(*         erewrite add_external_globals_pres_find_symbol; eauto. *)
+(*         unfold Genv.find_symbol. cbn. rewrite <- IDEQ. eauto. *)
+(*         rewrite <- IDEQ. eapply norepet_only_internal_symbol; eauto. *)
+(*       *  *)
+(*         unfold symbtable_to_idlist in GET'. *)
+(*         rewrite in_map_iff in GET'. *)
+(*         destruct GET' as (e' & EQ' & IN). inversion EQ'. subst e'. *)
+(*         erewrite add_external_globals_find_symb; eauto. *)
+(*         erewrite acc_symb_pres_ids in wf_prog_norepet_defs; eauto. *)
+(*         subst e. erewrite <- get_symbentry_pres_internal_prop. auto. *)
+(*     } *)
+(*     destruct FIND' as (b' & ofs' & FIND'). *)
+(*     exists b', ofs'. split; auto. unfold tge in FIND'. rewrite FIND'. auto. *)
+
+(*   - (* agree_inj_ext_funct *) *)
+(*     intros b f ofs b' FPTR INITINJ. *)
+(*     unfold init_meminj in INITINJ.  *)
+(*     destruct eq_block. inv INITINJ. *)
+(*     unfold ge in FPTR. exploit Genv.genv_next_find_funct_ptr_absurd; eauto. contradiction. *)
+(*     destr_match_in INITINJ; try congruence. *)
+(*     destr_match_in INITINJ; try congruence. *)
+(*     destruct p. inversion INITINJ. clear INITINJ. subst b0 ofs.  *)
+(*     rewrite Ptrofs.repr_unsigned. *)
+(*     apply Genv.invert_find_symbol in EQ. *)
+(*     exploit Genv.find_symbol_funct_ptr_inversion; eauto. *)
+(*     intros IN. *)
+(*     inversion w. *)
+(*     exploit PTree_Properties.of_list_norepet; eauto. *)
+(*     intros GET. *)
+(*     unfold gen_symb_table in Heqp. destr_in Heqp. *)
+(*     destruct p. destruct p. *)
+(*     inversion Heqp. subst l z0 z. *)
+(*     exploit acc_symb_tree_entry_some; eauto. *)
+(*     intros GET'.      *)
+(*     cbn in GET'. *)
+(*     unfold globalenv in tge; cbn in tge. *)
+(*     unfold tge. *)
+(*     unfold symbtable_to_tree in GET'. *)
+(*     apply PTree_Properties.in_of_list in GET'. *)
+(*     match type of GET' with *)
+(*     | In (_, ?e') _ => set (e:= e') in GET' *)
+(*     end. *)
+(*     unfold globalenv in EQ0; simpl in EQ0. *)
+(*     replace (prog_symbtable tprog) with (rev s) in * by (subst tprog; auto). *)
+(*     replace (prog_defs tprog) with (AST.prog_defs prog) in * by (subst tprog; auto). *)
+(*     cbn. *)
+(*     unfold symbtable_to_idlist in GET'. *)
+(*     rewrite in_map_iff in GET'. *)
+(*     destruct GET' as (e' & EQ' & IN'). inversion EQ'. clear EQ'. subst e'. *)
+(*     erewrite <- H0 in EQ0. *)
+(*     erewrite add_external_globals_find_symb in EQ0; eauto.  *)
+(*     inversion EQ0; clear EQ0. subst i0 b'. *)
+(*     rewrite <- H0. *)
+(*     assert ((gen_extfuns (AST.prog_defs prog)) ! (symbentry_id e) = Some f) as EXT. *)
+(*     {  *)
+(*       rewrite H0.  *)
+(*       eapply PTree_Properteis_of_list_get_extfuns; eauto.       *)
+(*     } *)
+(*     match goal with  *)
+(*     | [ |- context [ add_external_globals _ ?ge _ ] ] => set (ige := ge) *)
+(*     end. *)
+(*     erewrite acc_symb_pres_ids in wf_prog_norepet_defs; eauto. *)
+(*     assert (is_symbentry_internal e = false) as INT by auto. *)
+(*     assert (symbentry_type e = symb_func) as TYP by auto. *)
+(*     generalize (add_external_globals_ext_funs _ _ ige _ _ wf_prog_norepet_defs IN' INT TYP EXT). *)
+(*     intros EGET. rewrite <- EGET. *)
+(*     repeat f_equal. *)
+(*     erewrite <- acc_symb_pres_ids; eauto.     *)
+
+(*   - (* agree_inj_int_funct *) *)
+(*     intros b f ofs b' ofs' FPTR INITINJ. *)
+(*     unfold init_meminj in INITINJ.  *)
+(*     destruct eq_block. inv INITINJ. *)
+(*     unfold ge in FPTR. exploit Genv.genv_next_find_funct_ptr_absurd; eauto. contradiction. *)
+(*     destr_match_in INITINJ; try congruence. *)
+(*     destr_match_in INITINJ; try congruence. *)
+(*     destruct p. inversion INITINJ. clear INITINJ. subst b0 ofs.  *)
+(*     apply Genv.invert_find_symbol in EQ. *)
+(*     exploit Genv.find_symbol_funct_ptr_inversion; eauto. *)
+(*     intros IN. *)
+(*     inversion w. *)
+(*     exploit PTree_Properties.of_list_norepet; eauto. *)
+(*     intros GET. *)
+(*     generalize Heqp. intros GENSYM. *)
+(*     unfold gen_symb_table in Heqp. destr_in Heqp. *)
+(*     destruct p. destruct p. *)
+(*     inversion Heqp. subst l z0 z z1. *)
+(*     exploit acc_symb_tree_entry_some; eauto. *)
+(*     intros GET'.      *)
+(*     cbn in GET'. *)
+(*     unfold globalenv in tge; cbn in tge. *)
+(*     unfold tge. *)
+(*     unfold symbtable_to_tree in GET'. *)
+(*     apply PTree_Properties.in_of_list in GET'. *)
+(*     match type of GET' with *)
+(*     | In (_, ?e') _ => set (e:= e') in GET' *)
+(*     end. *)
+(*     unfold globalenv in EQ0; simpl in EQ0. *)
+(*     replace (prog_symbtable tprog) with (rev s) in * by (subst tprog; auto). *)
+(*     replace (prog_defs tprog) with (AST.prog_defs prog) in * by (subst tprog; auto). *)
+(*     cbn. *)
+(*     unfold symbtable_to_idlist in GET'. *)
+(*     rewrite in_map_iff in GET'. *)
+(*     destruct GET' as (e' & EQ' & IN'). inversion EQ'. clear EQ'. subst e'. *)
+(*     erewrite <- H0 in EQ0. *)
+(*     rewrite add_external_globals_pres_find_symbol in EQ0. *)
+(*     unfold Genv.find_symbol in EQ0. cbn in EQ0. *)
+(*     erewrite add_external_globals_pres_ext_funs; eauto.  *)
+(*     cbn. rewrite PTree.gempty. auto. cbn.     *)
+(*     eapply gen_symb_map_internal_block_range; eauto.  *)
+(*     erewrite <- acc_symb_pres_ids; eauto. *)
+(*     subst e. auto.  *)
+(*     subst e. auto. *)
+(*     cbn; auto.  *)
+(*     unfold sec_code_id. xomega. *)
+(*     eapply gen_symb_table_only_internal_symbol; eauto. *)
+(*     cbn. auto. *)
+(* Qed. *)
+
+
+(** Initial memory injection for global variables (not including the stacks) *)
+(* Definition globs_meminj : meminj := *)
+(*   let ge := Genv.globalenv prog in *)
+(*   let tge := globalenv tprog in *)
+(*   fun b => *)
+(*       match (Genv.invert_symbol ge b) with *)
+(*       | None => None *)
+(*       | Some id => *)
+(*         match Genv.find_symbol tge id with *)
+(*         | None => None *)
+(*         | Some (b, ofs) => Some (b, Ptrofs.unsigned ofs) *)
+(*         end *)
+(*       end. *)
+
+Lemma init_mem_inj_1:
+  Mem.mem_inj (Mem.flat_inj (Mem.support m)) m tm.
+Admitted.
+
+Lemma init_mem_inj_2:
+  Mem.inject (Mem.flat_inj (Mem.support m)) m tm.
+Admitted.
+
+Lemma alloc_stack_pres_inject:
+  forall lo hi stk stk' j m' tm',
+    Mem.alloc m lo hi = (m', stk) ->
+    Mem.alloc tm lo hi = (tm', stk') ->
+    j = (Mem.flat_inj (Mem.support m')) ->
+    Mem.inject j m' tm' /\ stk = stk' /\ match_inj j.
+Admitted.
+
+
+End INIT_MEM.
+
+(* Need preserve match_inj lemma after store*)
+Lemma storev_pres_match_inj:
+  forall chunk m m' addr v,
+    Mem.storev chunk m addr v = Some m' ->
+    match_inj (Mem.flat_inj (Mem.support m)) ->
+    match_inj (Mem.flat_inj (Mem.support m')).
+Admitted.
+
+Lemma storev_pres_inject:
+  forall chunk j m1 m1' m2 a a' v v',
+    Mem.storev chunk m1 a v = Some m2 ->
+    Mem.inject j m1 m1' ->
+    Val.inject j v v' ->
+    Val.inject j a a' ->
+    j = (Mem.flat_inj (Mem.support m1)) ->
+    exists m2',  Mem.storev chunk m1' a' v' = Some m2' /\ Mem.inject (Mem.flat_inj (Mem.support m2)) m2 m2'.
+Admitted.
+
+  
+Lemma init_mem_exists:
+  forall m, Genv.init_mem prog = Some m ->
+  exists tm, init_mem instr_size tprog = Some tm.
+Proof.
+Admitted.
+
+
+Lemma init_mem_pres_inject :
+  forall m
+    (INITMEM: Genv.init_mem prog = Some m),
+  exists m', init_mem instr_size tprog = Some m' /\ Mem.inject (Mem.flat_inj (Mem.support m)) m m'.
+  Admitted.
+(* Proof. *)
+(*   Admitted. *)
+(***** Remove Proofs By Chris Start ******)
+(*  
+  unfold Genv.init_mem, init_mem. intros.
+  unfold match_prog, transf_program in TRANSF.
+  destr_in TRANSF. inv w.
+  destr_in TRANSF. destruct p. destruct p.
+  destr_in TRANSF. inv TRANSF. cbn.
+  destruct (Mem.alloc Mem.empty 0 (init_data_list_size (fold_right acc_init_data [] (AST.prog_defs prog)))) eqn:IALLOC.
+  set (idata := (fold_right acc_init_data [] (AST.prog_defs prog))) in *.
+  generalize (alloc_perm_range _ _ _ _ _ Cur Freeable IALLOC).
+  intros RPERM.
+  assert (exists m1, store_zeros m0 b 0 (init_data_list_size idata) = Some m1) as STZ.
+  { 
+    eapply Genv.store_zeros_exists; eauto.
+    eapply Mem.range_perm_implies; eauto. constructor.
+    cbn. erewrite Mem.alloc_stack_blocks; eauto.
+    rewrite Mem.empty_stack. 
+    eapply stack_access_nil.
+    erewrite Mem.alloc_stack_blocks; eauto.
+    rewrite Mem.empty_stack. cbn. auto.
+  }
+  destruct STZ as (m1 & STZ).
+  rewrite STZ.
+  generalize (store_zeros_pres_range_perm _ _ _ _ _ _ _ STZ RPERM).
+  intros RPERM1.
+  
+  assert (exists m' : mem, store_init_data_list tge m1 b 0 idata = Some m') as SL.
+  {
+    eapply store_init_data_list_exists; eauto. cbn.
+    eapply Mem.range_perm_implies; eauto. constructor.
+    erewrite Genv.store_zeros_stack_access; eauto.
+    erewrite Mem.alloc_stack_blocks; eauto.
+    rewrite Mem.empty_stack.
+    apply stack_access_nil.
+    eapply acc_init_data_list_aligned; eauto.
+    eapply init_mem_data_aligned; eauto.
+    apply Z.divide_0_r.
+  }
+  destruct SL as (m2 & SL).
+  generalize SL. intros SL'.
+  unfold tge in SL'. cbn in SL'.
+  rewrite SL'. clear SL'.
+
+(*   destr. *)
+(*   destr. destr. *)
+
+(*   destruct (Mem.alloc Mem.empty 0 0) eqn:IALLOC. *)
+(*   exploit Mem.nextblock_alloc; eauto. intros NEXTBLOCK. *)
+(*   rewrite Mem.nextblock_empty in NEXTBLOCK. simpl in NEXTBLOCK. *)
+(*   exploit alloc_globals_segments_weak_inject; eauto. *)
+(*   erewrite Mem.alloc_stack_blocks; eauto. *)
+(*   erewrite Mem.empty_stack; eauto. *)
+(*   intros (m' & GALLOC & SINJ). *)
+(*   set (m1 := alloc_segments m0 (list_of_segments tprog)) in *. *)
+(*   rewrite GALLOC. *)
+(*   generalize (store_all_globals_inject). intro AAGI. *)
+(*   generalize TRANSF. intros TRANSF'. unfold match_prog in TRANSF'. *)
+(*   unfold transf_program in TRANSF'. *)
+(*   destruct (check_wellformedness prog) eqn:WF; try congruence. repeat destr_in TRANSF'. *)
+(*   unfold transl_prog_with_map in H0.  *)
+(*   destruct (transl_globdefs g (AST.prog_defs prog)) eqn: TLGLB; inversion H0.  *)
+(*   clear H0. simpl. *)
+(*   inversion UPDATE. subst g l z0 z. *)
+(*   exploit AAGI; eauto using INITMEM, SINJ, Mem.inject_ext. *)
+(*   - inv w. auto. *)
+(*   - erewrite alloc_globals_nextblock; eauto. *)
+(*     subst m1. *)
+(*     erewrite alloc_segments_nextblock; eauto. *)
+(*     erewrite Mem.nextblock_alloc; eauto.  *)
+(*     erewrite Mem.nextblock_empty. simpl.     *)
+(*     subst tprog. simpl. *)
+(*     erewrite transl_globdefs_pres_len; eauto. *)
+(*   - erewrite <- alloc_globals_stack; eauto. *)
+(*     subst m1. erewrite alloc_segments_stack; eauto. *)
+(*     erewrite Mem.alloc_stack_blocks; eauto. *)
+(*     erewrite Mem.empty_stack; eauto. *)
+(*   - eapply alloc_globals_perm_ofs; eauto. subst m1. *)
+(*     eapply alloc_segments_perm_ofs; eauto.  *)
+(*     intros b0 ofs k p PERM. erewrite alloc_perm in PERM; eauto. *)
+(*     destruct peq. omega. apply Mem.perm_empty in PERM. contradiction. *)
+(*   - intros id odef b' delta IN FSYM ofs k p OFS. *)
+(*     destruct (vit_dec _ _ odef). *)
+(*     + eapply alloc_globals_pres_perm; eauto. *)
+(*       subst m1. eapply alloc_segments_init_perm; eauto. *)
+(*     + eapply alloc_globals_init_perm; eauto. *)
+(*       subst m1. erewrite alloc_segments_nextblock; eauto. simpl. *)
+(*       rewrite NEXTBLOCK. auto. *)
+(*   - intros (m1' & ALLOC' & MINJ). *)
+(*     exists m1'. split. subst. simpl. *)
+(*     unfold tge in ALLOC'. auto. *)
+(*     auto. *)
+(* Qed. *)
+Admitted.
+*)
+(***** Remove Proofs By Chris End ******)
+
+(** Inversion of initial memory injection on genv_next *)
+(* Lemma acc_symb_maps_inv : forall stbl t id b ofs, *)
+(*     t ! id = None -> *)
+(*     (fold_right acc_symb_map t stbl) ! id = Some (b, ofs) -> *)
+(*     exists e, In e stbl /\  *)
+(*          id = symbentry_id e /\  *)
+(*          (exists i, symbentry_secindex e = secindex_normal i /\ *)
+(*                b = sec_index_to_block i) /\ *)
+(*          ofs = Ptrofs.repr (symbentry_value e). *)
+(* Proof. *)
+(*   induction stbl as [|e stbl]. *)
+(*   - intros. cbn in *. congruence. *)
+(*   - intros t id b ofs NON ACC. cbn in ACC. *)
+(*     unfold acc_symb_map in ACC. *)
+(*     destr_in ACC. *)
+(*     + destruct (peq (symbentry_id e) id). *)
+(*       * subst. rewrite PTree.gss in ACC. inv ACC. *)
+(*         eexists. intuition. eauto. *)
+(*       * rewrite PTree.gso in ACC; auto. *)
+(*         exploit IHstbl; eauto. *)
+(*         intros (e' & IN & ID & (i & SI & BL) & OFS). *)
+(*         subst.  *)
+(*         exists e'. split; eauto. *)
+(*     + exploit IHstbl; eauto. *)
+(*       intros (e' & IN & ID & (i & SI & BL) & OFS). *)
+(*       subst.  *)
+(*       exists e'. split; eauto. *)
+(*     + exploit IHstbl; eauto. *)
+(*       intros (e' & IN & ID & (i & SI & BL) & OFS). *)
+(*       subst.  *)
+(*       exists e'. split; eauto. *)
+(* Qed.         *)
+
+(* Lemma gen_symb_table_index_range: forall rdid did cid p stbl rdz dz cz e i, *)
+(*     gen_symb_table rdid did cid p = (stbl, rdz, dz, cz) -> *)
+(*     In e stbl ->  *)
+(*     symbentry_secindex e = secindex_normal i -> *)
+(*     i = rdid \/ i = did \/ i = cid. *)
+(* Proof. *)
+(*   intros rdid did cid p stbl rdz dz cz e i GEN IN SI. *)
+(*   unfold gen_symb_table in GEN. *)
+(*   destr_in GEN. destruct p0. destruct p0. inv GEN. *)
+(*   exploit acc_symb_index_in_range; eauto. *)
+(*   intros RNG. red in RNG. *)
+(*   rewrite Forall_forall in RNG.  *)
+(*   apply RNG in IN. red in IN.  *)
+(*   rewrite SI in IN. inv IN; auto. inv H; auto. inv H0; auto. inv H. *)
+(* Qed. *)
+
+
+(* Lemma find_symbol_globenv_block_bound : *)
+(*   forall (id : ident) b ofs, Genv.find_symbol (globalenv tprog) id = Some (b, ofs)  *)
+(*                         -> Pos.lt b (Genv.genv_next (globalenv tprog)). *)
+(* Proof. *)
+(*   unfold globalenv. simpl. intros. *)
+(*   exploit add_external_globals_pres_find_symbol_block_bound; eauto.  *)
+(*   red. simpl. intros. *)
+(*   unfold match_prog in TRANSF. unfold transf_program in TRANSF. *)
+(*   repeat destr_in TRANSF. cbn in H0. *)
+(*   clear H.  *)
+(*   unfold Genv.find_symbol in H0. cbn in H0. *)
+(*   exploit acc_symb_maps_inv; eauto. *)
+(*   apply PTree.gempty. *)
+(*   intros (e & IN & ID & (i & SI & BL) & OFS). subst. *)
+(*   exploit gen_symb_table_index_range; eauto. *)
+(*   intros [I | I]; subst; cbn. xomega. *)
+(*   destruct I; subst; cbn; xomega. *)
+(* Qed. *)
+
+(* Lemma init_meminj_genv_next_inv : forall b delta *)
+(*     (MINJ: init_meminj b = Some (Genv.genv_next tge, delta)), *)
+(*     b = Globalenvs.Genv.genv_next ge. *)
+(* Proof. *)
+(*   intros. *)
+(*   unfold init_meminj in MINJ. destruct eq_block; inv MINJ. *)
+(*   - unfold ge. auto. *)
+(*   - destr_match_in H0; inv H0. *)
+(*     destr_match_in H1; inv H1. *)
+(*     destruct p. inv H0. *)
+(*     exploit find_symbol_globenv_block_bound; eauto. *)
+(*     intros. *)
+(*     exfalso. generalize H. *)
+(*     setoid_rewrite <- Pos.compare_nlt_iff. *)
+(*     apply Pos.lt_irrefl. *)
+(* Qed. *)
+
+(** Injection of main pointer *)
+(***** Remove Proofs By Chris Start ******)
+(* Main Function 
+Lemma main_ptr_inject:
+  forall (MATCH_INJ: match_inj init_meminj),
+    Val.inject init_meminj
+               (Globalenvs.Genv.symbol_address
+                  (Globalenvs.Genv.globalenv prog)
+                  (AST.prog_main prog) Ptrofs.zero)
+               (Genv.symbol_address
+                  (globalenv tprog)
+                  (prog_main tprog) Ptrofs.zero).
+Proof.
+  intros.
+  unfold match_prog in TRANSF. unfold transf_program in TRANSF.
+  repeat destr_in TRANSF. destruct p. inv Heqp0. monadInv TRANSF.
+  cbn [prog_main].
+  rewrite H0. clear H0.
+  inv w. auto.
+  red in wf_prog_main_exists. rewrite Exists_exists in wf_prog_main_exists.
+  destruct wf_prog_main_exists as (def & IN & P).
+  destruct def. (* destruct o; destruct P as [IDEQ P]; *) inv P.
+  cbn [prog_main].
+  eapply symbol_address_inject; eauto.
+Qed.
+*)
+(***** Remove Proofs By Chris End ******)
+
+Lemma val_inject_set:
+  forall j rs1 rs2
+    (RINJ: forall r, Val.inject j (rs1 r) (rs2 r))
+    v v' (VINJ: Val.inject j v v') r1 r,
+    Val.inject j ((rs1 # r1 <- v) r) ((rs2 # r1 <- v') r).
+Proof.
+  intros.
+  destruct (PregEq.eq r1 r); subst; auto.
+  rewrite ! Pregmap.gss; auto.
+  rewrite ! Pregmap.gso by auto. auto.
+Qed.
+
+Lemma transf_initial_states : forall rs st1,
+    RealAsm.initial_state prog st1 ->
+    exists st2, initial_state instr_size tprog rs st2 /\ match_states st1 st2.
+Proof.  
+  intros rs st1 INIT.
+  generalize TRANSF. intros TRANSF'.
+  unfold match_prog in TRANSF'. unfold transf_program in TRANSF'.
+  destruct (check_wellformedness prog) eqn:WF. 2: congruence. destr_in TRANSF'. 
+  inv INIT.
+  exploit (init_mem_pres_inject m0);eauto.
+  intros (m0' & INITM' & MINJ).
+  (* exploit (Mem.alloc_parallel_inject (Mem.flat_inj (Mem.support m0)) *)
+  (*              m0 m0' 0 (max_stacksize + align (size_chunk Mptr) 8) *)
+  (*              m1 stk 0 (max_stacksize + align (size_chunk Mptr) 8));eauto;try lia. *)
+  exploit (Mem.valid_new_block m0);eauto. unfold Mem.valid_block. intros VALIDSTK.
+  caseEq (Mem.alloc m0' 0 (max_stacksize + align (size_chunk Mptr) 8)).
+  intros m1'  stk'  H0'.
+  exploit (alloc_stack_pres_inject m0 m0');eauto.
+  intros (MINJ1 &  STK &  MATINJ1). subst.  
+  exploit (storev_pres_match_inj Mptr m1 m2);eauto.
+  intros MATINJ2.
+  edestruct storev_pres_inject as (m2' & ST & SMINJ). apply H1. apply MINJ1. econstructor. econstructor.
+  (* stk' is valid *)
+  unfold Mem.flat_inj. destruct (Mem.sup_dec stk' (Mem.support m1)).
+  eauto. congruence.
+  eapply eq_refl. constructor.
+  (* regset *)
+  set (rs0' := rs # PC <- (Genv.symbol_address tge tprog.(prog_main) Ptrofs.zero)
+           # RA <- Vnullptr
+           # RSP <- (Vptr stk' (Ptrofs.sub (Ptrofs.repr (max_stacksize + align (size_chunk Mptr) 8)) (Ptrofs.repr (size_chunk Mptr))))) in *.
+
+  (* instantiate the initial state*)
+  exists (State rs0' m2').
+  split. 
+  (* initial_state *)
+  - econstructor;eauto.
+    econstructor;eauto.
+  - econstructor;eauto.
+    unfold regset_inject. intros.
+    
+    unfold rs0',rs0.
+    apply val_inject_set.
+    apply val_inject_set.
+    apply val_inject_set.
+    auto.
+      (* main function *)
+      destr_in TRANSF'. simpl.
+     exploit (agree_inj_globs (Mem.flat_inj (Mem.support m2)) MATINJ2 ((AST.prog_main prog)) bmain). auto.
+     intros (bmain' & ofs' & MAIN' & MAININJ).
+     (* proof bmain is valid in m2 support *)
+     exploit (Genv.find_symbol_not_fresh). apply H. apply H2. intros VALIDMAIN0.
+     exploit (Mem.valid_block_alloc). apply H0. apply VALIDMAIN0. intros VALIDMAIN1.
+     exploit (Mem.support_store). apply H1. intros SUPEQ.
+     unfold Mem.valid_block in VALIDMAIN1.
+     rewrite <- SUPEQ in VALIDMAIN1. unfold Mem.flat_inj in MAININJ.
+     destruct (Mem.sup_dec bmain (Mem.support m2));try congruence.
+     destr_in MAININJ.
+     unfold Genv.symbol_address.
+     rewrite MAIN'. econstructor.
+     unfold Mem.flat_inj. destruct (Mem.sup_dec bmain' (Mem.support m2));try congruence. eauto.
+     rewrite Ptrofs.add_unsigned. rewrite Ptrofs.add_zero.
+     rewrite <- H6. rewrite Z.add_0_r. rewrite Ptrofs.unsigned_zero. auto.
+     constructor.
+     admit.
+
+     (* glob_block_valid *)
+     admit.
+Admitted.
+  
+(* Lemma transf_initial_states : forall rs (SELF: forall j, forall r : PregEq.t, Val.inject j (rs r) (rs r)) st1, *)
+(*     RealAsm.initial_state prog rs st1  -> *)
+(*     exists st2, initial_state tprog rs st2 /\ match_states st1 st2. *)
+(* Proof. *)
+(*   intros rs SELFINJECT st1 INIT. *)
+(*   generalize TRANSF. intros TRANSF'. *)
+(*   unfold match_prog in TRANSF'. unfold transf_program in TRANSF'. *)
+(*   destruct (check_wellformedness prog) eqn:WF. 2: congruence. repeat destr_in TRANSF'. *)
+(*   rename z0 into dsize. rename z into csize.  *)
+(*   inv INIT. *)
+(*   generalize init_meminj_match_sminj. *)
+(*   intros MATCH_SMINJ. *)
+(*   exploit (init_mem_pres_inject m); eauto. *)
+(*   intros (m' & INITM' & MINJ). *)
+(*   inversion H0. *)
+(*   (* push_new stage *) *)
+(*   exploit Mem.push_new_stage_inject; eauto. intros NSTGINJ. *)
+(*   exploit (Mem.alloc_parallel_inject globs_meminj (1%nat :: def_frame_inj m) *)
+(*           (Mem.push_new_stage m) (Mem.push_new_stage m') *)
+(*           0 (Mem.stack_limit + align (size_chunk Mptr) 8) m1 bstack *)
+(*           0 (Mem.stack_limit + align (size_chunk Mptr) 8)); eauto. omega. omega. *)
+(*   intros (j' & m1' & bstack' & MALLOC' & AINJ & INCR & FBSTACK & NOTBSTK). *)
+(*   rewrite <- push_new_stage_def_frame_inj in AINJ. *)
+(*   erewrite alloc_pres_def_frame_inj in AINJ; eauto. *)
+(*   assert (bstack = Globalenvs.Genv.genv_next ge). *)
+(*   { *)
+(*     exploit (Genv.init_mem_genv_next prog m); eauto. intros BEQ. unfold ge. rewrite BEQ. *)
+(*     apply Mem.alloc_result in MALLOC; eauto. *)
+(*   } *)
+(*   assert (bstack' = Genv.genv_next tge). *)
+(*   { *)
+(*     exploit init_mem_genv_next; eauto. intros BEQ. *)
+(*     unfold tge. rewrite BEQ. *)
+(*     exploit Mem.alloc_result; eauto. *)
+(*   } *)
+(*   assert (forall x, j' x = init_meminj x). *)
+(*   { *)
+(*     intros. destruct (eq_block x bstack). *)
+(*     subst x. rewrite FBSTACK. unfold init_meminj. subst. *)
+(*     rewrite dec_eq_true; auto. *)
+(*     erewrite NOTBSTK; eauto. *)
+(*     unfold init_meminj. subst. *)
+(*     rewrite dec_eq_false; auto. *)
+(*   } *)
+(*   exploit Mem.inject_ext; eauto. intros MINJ'. *)
+(*   exploit drop_parallel_inject; eauto.  *)
+(*   unfold init_meminj. fold ge. rewrite <- H3. rewrite pred_dec_true. eauto. auto. *)
+(*   intros (m2' & MDROP' & DMINJ). simpl in MDROP'. rewrite Z.add_0_r in MDROP'. *)
+(*   erewrite (drop_perm_pres_def_frame_inj m1) in DMINJ; eauto. *)
+  
+(*   assert (exists m3', Mem.record_stack_blocks m2' (make_singleton_frame_adt' bstack' RawAsm.frame_info_mono 0) = Some m3' *)
+(*                  /\ Mem.inject (init_meminj) (def_frame_inj m3) m3 m3') as RCD. *)
+(*   { *)
+(*     unfold def_frame_inj. unfold def_frame_inj in DMINJ. *)
+(*     eapply (record_stack_block_inject_flat m2 m3 m2' (init_meminj) *)
+(*            (make_singleton_frame_adt' bstack RawAsm.frame_info_mono 0)); eauto. *)
+(*     (* frame inject *) *)
+(*     red. unfold make_singleton_frame_adt'. simpl. constructor. *)
+(*     simpl. intros b2 delta FINJ. *)
+(*     unfold init_meminj in FINJ. fold ge in FINJ. rewrite <- H3 in FINJ. *)
+(*     rewrite pred_dec_true in FINJ; auto. inv FINJ. *)
+(*     exists RawAsm.frame_info_mono. split. auto. apply inject_frame_info_id. *)
+(*     constructor. *)
+(*     (* in frame *) *)
+(*     unfold make_singleton_frame_adt'. simpl. unfold in_frame. simpl. *)
+(*     repeat rewrite_stack_blocks. *)
+(*     erewrite init_mem_stack; eauto. *)
+(*     (* valid frame *) *)
+(*     unfold make_singleton_frame_adt'. simpl. red. unfold in_frame. *)
+(*     simpl. intuition. subst. *)
+(*     eapply Mem.drop_perm_valid_block_1; eauto. *)
+(*     eapply Mem.valid_new_block; eauto. *)
+(*     (* frame_agree_perms *) *)
+(*     red. unfold make_singleton_frame_adt'. simpl. *)
+(*     intros b fi o k p BEQ PERM. inv BEQ; try contradiction. *)
+(*     inv H6. unfold RawAsm.frame_info_mono. simpl. *)
+(*     erewrite Mem.drop_perm_perm in PERM; eauto. destruct PERM. *)
+(*     eapply Mem.perm_alloc_3; eauto. *)
+(*     (* in frame iff *) *)
+(*     unfold make_singleton_frame_adt'. unfold in_frame. simpl. *)
+(*     intros b1 b2 delta INJB. split. *)
+(*     intros BEQ. destruct BEQ; try contradiction. subst b1. *)
+(*     unfold init_meminj in INJB. fold ge in INJB. rewrite <- H3 in INJB. *)
+(*     rewrite pred_dec_true in INJB; auto. inv INJB. left; auto. *)
+(*     intros BEQ. destruct BEQ; try contradiction. subst b2. *)
+(*     assert (bstack' = Mem.nextblock (Mem.push_new_stage m')) as BEQ. *)
+(*     eapply Mem.alloc_result; eauto using MALLOC'. *)
+(*     rewrite Mem.push_new_stage_nextblock in BEQ. *)
+(*     erewrite <- init_mem_genv_next in BEQ; eauto using INITM'. *)
+(*     subst bstack'. *)
+(*     destruct (eq_block bstack b1); auto. *)
+(*     assert (b1 <> bstack) by congruence. *)
+(*     apply NOTBSTK in H4. rewrite H5 in H4. rewrite INJB in H4. *)
+(*     left. symmetry. subst bstack. eapply init_meminj_genv_next_inv; eauto. *)
+
+(*     (* top frame *) *)
+(*     red. repeat rewrite_stack_blocks. constructor. auto. *)
+(*     (* size stack *) *)
+(*     repeat rewrite_stack_blocks. *)
+(*     erewrite init_mem_stack; eauto. simpl. omega. *)
+(*   } *)
+
+(*   destruct RCD as (m3' & RCDSB & RMINJ). *)
+(*   set (rs0' := rs # PC <- (Genv.symbol_address tge tprog.(prog_main) Ptrofs.zero) *)
+(*                   # RA <- Vnullptr *)
+(*                   # RSP <- (Vptr bstack' (Ptrofs.sub (Ptrofs.repr (Mem.stack_limit + align (size_chunk Mptr) 8)) (Ptrofs.repr (size_chunk Mptr))))) in *. *)
+(*   edestruct storev_mapped_inject' as (m4' & ST & SMINJ). apply RMINJ. eauto. econstructor. *)
+(*   rewrite <- H5, FBSTACK; eauto. reflexivity. constructor. *)
+(*   exists (State rs0' m4'). split. *)
+(*   - eapply initial_state_intro; eauto. *)
+(*     eapply initial_state_gen_intro; eauto. *)
+(*     subst. fold tge in MDROP'. eauto. *)
+(*     subst. fold tge in MDROP'. rewrite Ptrofs.add_zero in ST. eauto. *)
+(*   - eapply match_states_intro; eauto. *)
+(*     (* + eapply valid_instr_offset_is_internal_init; eauto. inv w; auto. *) *)
+(*     (* + eapply extfun_entry_is_external_init; eauto. inv w; auto. *) *)
+(*     (* + red. *) *)
+(*     (*   intros. eapply extfun_transf; eauto. inv w; auto. *) *)
+(*     + red. unfold rs0, rs0'. *)
+(*       apply AsmFacts.val_inject_set. *)
+(*       apply AsmFacts.val_inject_set. *)
+(*       apply AsmFacts.val_inject_set. *)
+(*       auto. *)
+(*       admit. *)
+(* (***** Remove Proofs By Chris Start ******) *)
+(* (* MAIN Function Insertion *)
+(*       exploit (main_ptr_inject); eauto. unfold Globalenvs.Genv.symbol_address. *)
+(*       unfold ge, ge0 in *. rewrite H1. fold tge. auto. *)
+(* *)       *)
+(* (***** Remove Proofs By Chris End ******) *)
+(*       unfold Vnullptr. destr; auto. *)
+(*       econstructor. unfold init_meminj. subst bstack. fold ge. rewrite peq_true. subst bstack'.  fold tge. eauto. *)
+(*       rewrite Ptrofs.add_zero. *)
+(*       apply Ptrofs.sub_add_opp. *)
+(*     + red. intros b g FD. *)
+(*       unfold Genv.find_def in FD. eapply Genv.genv_defs_range in FD. *)
+(*       revert FD. red. rewnb. *)
+(*       fold ge. intros. xomega. *)
+(* Admitted. *)
+
+(** ** Simulation of Single Step Execution *)
+
+Lemma eval_builtin_arg_inject : forall j m m' rs rs' sp sp' arg varg
+    (MATCHINJ: match_inj j)                              
+    (MINJ: Mem.inject j m m')
+    (RSINJ: regset_inject j rs rs')
+    (VINJ: Val.inject j sp sp')
+    (EVALBI: Events.eval_builtin_arg ge rs sp m arg varg),
+    exists varg', eval_builtin_arg _ tge rs' sp' m' arg varg' /\
+             Val.inject j varg varg'.
+Proof.
+  unfold regset_inject.
+  induction arg; intros; inv EVALBI.
+  - eexists; split; auto. constructor.
+  - eexists; split; auto. constructor.
+  - eexists; split; auto. constructor.
+  - eexists; split; auto. constructor.
+  - eexists; split; auto. constructor.
+  - exploit Mem.loadv_inject; eauto.
+    apply Val.offset_ptr_inject; eauto.
+    intros (v2 & ML & VJ); auto.
+    eexists; split. constructor. apply ML. auto.
+  - eexists; split. constructor.
+    apply Val.offset_ptr_inject; eauto.
+  - exploit Mem.loadv_inject; eauto.
+    apply symbol_address_inject; eauto.
+    intros (v2 & ML & VJ); auto.
+    eexists; split. constructor. apply ML. auto.
+  - eexists; split. constructor.
+    apply symbol_address_inject; eauto.
+  - exploit IHarg1; eauto.
+    intros (varg1 & EVALBI1 & JB1).
+    exploit IHarg2; eauto.
+    intros (varg2 & EVALBI2 & JB2).
+    eexists; split. constructor; eauto.
+    apply Val.longofwords_inject; auto.
+  - exploit IHarg1; eauto.
+    intros (varg1 & EVALBI1 & JB1).
+    exploit IHarg2; eauto.
+    intros (varg2 & EVALBI2 & JB2).
+    destruct Archi.ptr64 eqn: PTR.
+    eexists; split. econstructor;eauto.
+    rewrite PTR. eapply Val.addl_inject;auto.
+    eexists; split. econstructor;eauto.
+    rewrite PTR. eapply Val.add_inject;auto.
+Qed.
+
+Lemma eval_builtin_args_inject : forall j m m' rs rs' sp sp' args vargs
+    (MATCHINJ: match_inj j)
+    (MINJ: Mem.inject j m m')
+    (RSINJ: regset_inject j rs rs')
+    (VINJ: Val.inject j sp sp')
+    (EVALBI: Events.eval_builtin_args ge rs sp m args vargs),
+    exists vargs', eval_builtin_args _ tge rs' sp' m' args vargs' /\
+             Val.inject_list j vargs vargs'.
+Proof.
+  induction args; intros; simpl; inv EVALBI.
+  - eexists. split. constructor. auto.
+  - exploit eval_builtin_arg_inject; eauto.
+    intros (varg' & EVARG & JB).
+    exploit IHargs; eauto.
+    intros (vargs' & EVARGS & JBS).
+    exists (varg' :: vargs'). split; auto.
+    unfold eval_builtin_args.
+    apply list_forall2_cons; auto.
+Qed.
+
+Lemma extcall_arg_inject : forall rs1 rs2 m1 m2 l arg1 j,
+    extcall_arg rs1 m1 l arg1 ->
+    Mem.inject j m1 m2 ->
+    regset_inject j rs1 rs2 ->
+    exists arg2,
+      Val.inject j arg1 arg2 /\
+      extcall_arg rs2 m2 l arg2.
+Proof.
+  intros. inv H.
+  - unfold regset_inject in *.
+    specialize (H1 (Asm.preg_of r)). eexists; split; eauto.
+    constructor.
+  - exploit Mem.loadv_inject; eauto.
+    apply Val.offset_ptr_inject. apply H1.
+    intros (arg2 & MLOADV & ARGINJ).
+    exists arg2. split; auto.
+    eapply extcall_arg_stack; eauto.
+Qed.
+
+Lemma extcall_arg_pair_inject : forall rs1 rs2 m1 m2 lp arg1 j,
+    extcall_arg_pair rs1 m1 lp arg1 ->
+    Mem.inject j m1 m2 ->
+    regset_inject j rs1 rs2 ->
+    exists arg2,
+      Val.inject j arg1 arg2 /\
+      extcall_arg_pair rs2 m2 lp arg2.
+Proof.
+  intros. inv H.
+  - exploit extcall_arg_inject; eauto.
+    intros (arg2 & VINJ & EXTCALL).
+    exists arg2. split; auto. constructor. auto.
+  - exploit (extcall_arg_inject rs1 rs2 m1 m2 hi vhi); eauto.
+    intros (arghi & VINJHI & EXTCALLHI).
+    exploit (extcall_arg_inject rs1 rs2 m1 m2 lo vlo); eauto.
+    intros (arglo & VINJLO & EXTCALLLO).
+    exists (Val.longofwords arghi arglo). split.
+    + apply Val.longofwords_inject; auto.
+    + constructor; auto.
+Qed.
+
+Lemma extcall_arguments_inject_aux : forall rs1 rs2 m1 m2 locs args1 j,
+   list_forall2 (extcall_arg_pair rs1 m1) locs args1 ->
+    Mem.inject j m1 m2 ->
+    regset_inject j rs1 rs2 ->
+    exists args2,
+      Val.inject_list j args1 args2 /\
+      list_forall2 (extcall_arg_pair rs2 m2) locs args2.
+Proof.
+  induction locs; simpl; intros; inv H.
+  - exists nil. split.
+    + apply Val.inject_list_nil.
+    + unfold Asm.extcall_arguments. apply list_forall2_nil.
+  - exploit extcall_arg_pair_inject; eauto.
+    intros (arg2 & VINJARG2 & EXTCALLARG2).
+    exploit IHlocs; eauto.
+    intros (args2 & VINJARGS2 & EXTCALLARGS2).
+    exists (arg2 :: args2). split; auto.
+    apply list_forall2_cons; auto.
+Qed.
+
+Lemma extcall_arguments_inject : forall rs1 rs2 m1 m2 ef args1 j,
+    Asm.extcall_arguments rs1 m1 (ef_sig ef) args1 ->
+    Mem.inject j m1 m2 ->
+    regset_inject j rs1 rs2 ->
+    exists args2,
+      Val.inject_list j args1 args2 /\
+      Asm.extcall_arguments rs2 m2 (ef_sig ef) args2.
+Proof.
+  unfold Asm.extcall_arguments. intros.
+  eapply extcall_arguments_inject_aux; eauto.
+Qed.
+
+(* Lemma inject_pres_match_sminj :  *)
+(*   forall j j' m1 m2 (ms: match_inj j),  *)
+(*     glob_block_valid m1 -> inject_incr j j' -> inject_separated j j' m1 m2 ->  *)
+(*     match_inj j'. *)
+(* Proof. *)
+(*   unfold glob_block_valid. *)
+(*   intros. inversion ms. constructor; intros. *)
+(*   - *)
+(*     eapply (agree_inj_instrs0 b b'); eauto. *)
+(*     unfold Globalenvs.Genv.find_funct_ptr in H2. destruct (Globalenvs.Genv.find_def ge b) eqn:FDEF; try congruence. *)
+(*     exploit H; eauto. intros. *)
+(*     eapply inject_decr; eauto. *)
+(*   - *)
+(*     exploit agree_inj_globs0; eauto. *)
+(*     intros (b' & ofs' & GLBL & JB). *)
+(*     eexists; eexists; eexists; eauto. *)
+(*   - *)
+(*     eapply (agree_inj_ext_funct0 b); eauto. *)
+(*     unfold Globalenvs.Genv.find_funct_ptr in H2. destruct (Globalenvs.Genv.find_def ge b) eqn:FDEF; try congruence. *)
+(*     exploit H; eauto. intros. *)
+(*     eapply inject_decr; eauto. *)
+(*   -  *)
+(*     eapply (agree_inj_int_funct0 b); eauto. *)
+(*     unfold Globalenvs.Genv.find_funct_ptr in H2. destruct (Globalenvs.Genv.find_def ge b) eqn:FDEF; try congruence. *)
+(*     exploit H; eauto. intros. *)
+(*     eapply inject_decr; eauto. *)
+(* Qed. *)
+
+
+Lemma inject_symbol_address : forall j id ofs,
+    match_inj j ->
+    Val.inject j (Globalenvs.Genv.symbol_address ge id ofs) (Genv.symbol_address tge id ofs).
+Proof.
+  unfold Globalenvs.Genv.symbol_address.
+  intros.
+  destruct (Globalenvs.Genv.find_symbol ge id) eqn:FINDSYM; auto.
+  inv H. exploit agree_inj_globs0; eauto.
+  intros (b' & ofs' & SBOFS & JB).
+  erewrite Genv.symbol_address_offset; eauto. 
+  eapply Val.inject_ptr; eauto.
+  rewrite Ptrofs.repr_unsigned. apply Ptrofs.add_commut.
+  unfold Genv.symbol_address. rewrite SBOFS.
+  rewrite Ptrofs.add_zero_l. auto.
+Qed.
+
+
+Ltac simpl_goal :=
+  repeat match goal with
+         | [ |- context [ Int.add Int.zero _ ] ] =>
+           rewrite Int.add_zero_l
+         | [ |- context [ Int64.add Int64.zero _ ] ] =>
+           rewrite Int64.add_zero_l
+         | [ |- context [Ptrofs.add _ (Ptrofs.of_int Int.zero)] ] =>
+           rewrite Ptrofs.add_zero
+         | [ |- context [Ptrofs.add _ (Ptrofs.of_int64 Int64.zero)] ] =>
+           rewrite Ptrofs.add_zero
+         | [ |- context [Ptrofs.add Ptrofs.zero _] ] =>
+           rewrite Ptrofs.add_zero_l
+         | [ |- context [Ptrofs.repr (Ptrofs.unsigned _)] ] =>
+           rewrite Ptrofs.repr_unsigned
+         end.
+
+Ltac destr_pair_if :=
+  repeat match goal with
+         | [ |- context [match ?a with pair _ _ => _ end] ] =>
+           destruct a eqn:?
+         | [ |- context [if ?h then _ else _] ] =>
+           destruct h eqn:?
+         end.
+
+Ltac inject_match :=
+  match goal with
+  | [ |- Val.inject ?j (match ?a with _ => _ end) (match ?b with _ => _ end) ] =>
+    assert (Val.inject j a b)
+  end.
+
+Ltac inv_valinj :=
+  match goal with
+         | [ H : Val.inject _ (Vint _) _ |- _ ] =>
+           inversion H; subst
+         | [ H : Val.inject _ (Vlong _) _ |- _ ] =>
+           inversion H; subst
+         | [ H : Val.inject _ (Vptr _ _) _ |- _ ] =>
+           inversion H; subst
+         end.
+
+Ltac destr_valinj_right H :=
+  match type of H with
+  | Val.inject _ _ ?a =>
+    destruct a eqn:?
+  end.
+
+Ltac destr_valinj_left H :=
+  match type of H with
+  | Val.inject _ ?a ?b =>
+    destruct a eqn:?
+  end.
+
+Remark mul_inject:
+  forall f v1 v1' v2 v2',
+  Val.inject f v1 v1' ->
+  Val.inject f v2 v2' ->
+  Val.inject f (Val.mul v1 v2) (Val.mul v1' v2').
+Proof.
+  intros.
+  unfold Val.mul. destruct v1, v2; auto; inv H; inv H0; auto.
+Qed.
+
+
+Lemma eval_addrmode32_inject: forall j a rs1 rs2,
+    match_inj j ->
+    regset_inject j rs1 rs2 ->
+    Val.inject j (Asm.eval_addrmode32 ge a rs1) (eval_addrmode32 tge a rs2).
+Proof.
+  intros. unfold Asm.eval_addrmode32, eval_addrmode32.
+  destruct a. 
+  destruct base, ofs, const; simpl in *. 
+  - destruct p. repeat apply Val.add_inject; auto.
+    destr_pair_if; auto.
+    apply mul_inject; auto.
+  - destruct p,p0. repeat apply Val.add_inject; auto.
+    destr_pair_if; auto.
+    apply mul_inject; auto.
+    apply inject_symbol_address. auto.
+  - repeat apply Val.add_inject; auto.
+  - destruct p. apply Val.add_inject; auto. 
+    inject_match. apply inject_symbol_address; auto.
+    destr_valinj_left H1; inv H1; auto.
+    (* destr_pair_if. auto. *)
+    (* eapply Val.inject_ptr; eauto. *)
+    (* repeat unfold Ptrofs.of_int.  *)
+    (* repeat rewrite Int.unsigned_zero.  *)
+    (* repeat rewrite Ptrofs.add_zero. auto. *)
+  - destruct p.
+    inject_match.
+    apply Val.add_inject; auto.
+    destr_pair_if; auto.
+    apply mul_inject; auto.
+    destr_valinj_left H1; inv H1; auto.
+    (* destr_pair_if. auto. *)
+    (* eapply Val.inject_ptr; eauto. *)
+    (* repeat unfold Ptrofs.of_int.  *)
+    (* repeat rewrite Int.unsigned_zero.  *)
+    (* repeat rewrite Ptrofs.add_zero. auto. *)
+  - destruct p,p0.
+    inject_match.
+    apply Val.add_inject; auto.
+    destr_pair_if; auto.
+    apply mul_inject; auto.
+    apply inject_symbol_address; auto.
+    destr_valinj_left H1; inv H1; auto.
+    (* destr_pair_if. auto. *)
+    (* eapply Val.inject_ptr; eauto. *)
+    (* repeat unfold Ptrofs.of_int.  *)
+    (* repeat rewrite Int.unsigned_zero.  *)
+    (* repeat rewrite Ptrofs.add_zero. auto. *)
+  - repeat apply Val.add_inject; auto.
+  - destruct p. 
+    inject_match. inject_match.
+    apply inject_symbol_address; auto.
+    destr_valinj_left H1; inv H1; auto.
+    Admitted.
+    (* destr_pair_if. auto. *)
+    (* eapply Val.inject_ptr; eauto. *)
+    (* repeat unfold Ptrofs.of_int.  *)
+    (* repeat rewrite Int.unsigned_zero.  *)
+    (* repeat rewrite Ptrofs.add_zero. auto. *)
+    (* destr_valinj_left H1; inv H1; auto. *)
+    (* destr_pair_if. auto. *)
+    (* eapply Val.inject_ptr; eauto. *)
+    (* repeat unfold Ptrofs.of_int.  *)
+    (* repeat rewrite Int.unsigned_zero.  *)
+    (* repeat rewrite Ptrofs.add_zero. auto. *)   
+
+Lemma eval_addrmode64_inject: forall j a rs1 rs2,
+    match_inj j ->
+    regset_inject j rs1 rs2 ->
+    Val.inject j (Asm.eval_addrmode64 ge a rs1) (eval_addrmode64 tge a rs2).
+Proof.
+  intros. unfold Asm.eval_addrmode32, eval_addrmode32.
+  destruct a. 
+  destruct base, ofs, const; simpl in *.
+  - destruct p. repeat apply Val.addl_inject; auto.
+    destr_pair_if; auto.
+Admitted.
+
+(*     apply Val.mull_inject; auto. *)
+(*   - destruct p,p0. repeat apply Val.addl_inject; auto. *)
+(*     destr_pair_if; auto. *)
+(*     apply Val.mull_inject; auto. *)
+(*     apply inject_symbol_address. auto. *)
+(*   - repeat apply Val.addl_inject; auto. *)
+(*   - destruct p. apply Val.addl_inject; auto.  *)
+(*     inject_match. apply inject_symbol_address; auto. *)
+(*     destr_valinj_left H1; inv H1; auto. *)
+(*     (* destr_pair_if; auto. *) *)
+(*     (* eapply Val.inject_ptr; eauto.  *) *)
+(*     (* repeat rewrite Ptrofs.add_assoc.  *) *)
+(*     (* rewrite (Ptrofs.add_commut (Ptrofs.repr delta) (Ptrofs.of_int64 Int64.zero)). auto. *) *)
+(*   - destruct p.  *)
+(*     inject_match. *)
+(*     apply Val.addl_inject; auto. *)
+(*     destr_pair_if; auto.  *)
+(*     apply Val.mull_inject; auto. *)
+(*     destr_valinj_left H1; inv H1; auto. *)
+(*     (* destr_pair_if; auto. *) *)
+(*     (* eapply Val.inject_ptr; eauto.  *) *)
+(*     (* repeat rewrite Ptrofs.add_assoc.  *) *)
+(*     (* rewrite (Ptrofs.add_commut (Ptrofs.repr delta) (Ptrofs.of_int64 Int64.zero)). auto. *) *)
+(*   - destruct p,p0. *)
+(*     inject_match. *)
+(*     apply Val.addl_inject; auto. *)
+(*     destr_pair_if; auto.  *)
+(*     apply Val.mull_inject; auto. *)
+(*     apply inject_symbol_address; auto. *)
+(*     destr_valinj_left H1; inv H1; auto. *)
+(*     (* destr_pair_if; auto. *) *)
+(*     (* eapply Val.inject_ptr; eauto.  *) *)
+(*     (* repeat rewrite Ptrofs.add_assoc.  *) *)
+(*     (* rewrite (Ptrofs.add_commut (Ptrofs.repr delta) (Ptrofs.of_int64 Int64.zero)). auto. *) *)
+(*   - repeat apply Val.addl_inject; auto. *)
+(*   - destruct p. inject_match. inject_match. *)
+(*     apply inject_symbol_address; auto. *)
+(*     destr_valinj_left H1; inv H1; auto. *)
+(*     destr_valinj_left H1; inv H1; auto. *)
+(*     (* eapply Val.inject_ptr; eauto.  *) *)
+(*     (* repeat rewrite Ptrofs.add_assoc.  *) *)
+(*     (* rewrite (Ptrofs.add_commut (Ptrofs.repr delta) (Ptrofs.of_int64 Int64.zero)). auto. *)     *)
+(* Qed. *)
+
+Lemma eval_addrmode_inject: forall j a rs1 rs2,
+    match_inj j ->
+    regset_inject j rs1 rs2 ->
+    Val.inject j (Asm.eval_addrmode ge a rs1) (eval_addrmode tge a rs2).
+Proof.
+  intros. unfold Asm.eval_addrmode, eval_addrmode. destruct Archi.ptr64.
+  + eapply eval_addrmode64_inject; eauto.
+  + eapply eval_addrmode32_inject; eauto.
+Qed.
+
+
+Lemma exec_load_step: forall j rs1 rs2 m1 m2 rs1' m1' sz chunk rd a
+                          (MINJ: Mem.inject j  m1 m2)
+                          (MATCHINJ: match_inj j)
+                          (RSINJ: regset_inject j rs1 rs2)
+                          (GBVALID: glob_block_valid m1), 
+    Asm.exec_load ge sz chunk m1 a rs1 rd = Next rs1' m1' ->
+    exists rs2' m2',
+      exec_load sz tge chunk m2 a rs2 rd = Next rs2' m2' /\
+      match_states (State rs1' m1') (State rs2' m2').
+Proof.
+  intros. unfold Asm.exec_load in *.
+  exploit eval_addrmode_inject; eauto. intro EMODINJ.
+  destruct (Mem.loadv chunk m1 (Asm.eval_addrmode ge a rs1)) eqn:MLOAD; try congruence.
+  exploit Mem.loadv_inject; eauto. intros (v2 & MLOADV & VINJ).
+  eexists. eexists. split.
+  - unfold exec_load. rewrite MLOADV. auto.
+  - inv H. eapply match_states_intro; eauto.
+    apply nextinstr_pres_inject. apply undef_regs_pres_inject.
+    apply regset_inject_expand; eauto.
+Qed.
+
+Lemma store_pres_glob_block_valid : forall m1 chunk b v ofs m2,
+  Mem.store chunk m1 b ofs v = Some m2 -> glob_block_valid m1 -> glob_block_valid m2.
+Proof.
+  unfold glob_block_valid in *. intros.
+  eapply Mem.store_valid_block_1; eauto.
+Qed.
+
+Lemma storev_pres_glob_block_valid : forall m1 chunk ptr v m2,
+  Mem.storev chunk m1 ptr v = Some m2 -> glob_block_valid m1 -> glob_block_valid m2.
+Proof.
+  unfold Mem.storev. intros. destruct ptr; try congruence.
+  eapply store_pres_glob_block_valid; eauto.
+Qed.
+
+Lemma exec_store_step: forall j rs1 rs2 m1 m2 rs1' m1' sz chunk r a dregs
+                         (MINJ: Mem.inject j (def_frame_inj m1) m1 m2)
+                         (MATCHINJ: match_inj j)
+                         (RSINJ: regset_inject j rs1 rs2)
+                         (GBVALID: glob_block_valid m1),
+    Asm.exec_store ge chunk m1 a rs1 r dregs sz = Next rs1' m1' ->
+    exists rs2' m2',
+      exec_store tge chunk m2 a rs2 r dregs sz = Next rs2' m2' /\
+      match_states (State rs1' m1') (State rs2' m2').
+Proof.
+  intros. unfold Asm.exec_store in *.
+  exploit eval_addrmode_inject; eauto. intro EMODINJ.
+  destruct (Mem.storev chunk m1 (Asm.eval_addrmode ge a rs1) (rs1 r)) eqn:MSTORE; try congruence.
+  exploit Mem.storev_mapped_inject; eauto. intros (m2' & MSTOREV & MINJ').
+  eexists. eexists. split.
+  - unfold exec_store. rewrite MSTOREV. auto.
+  - inv H. eapply match_states_intro; eauto.
+    erewrite <- storev_pres_def_frame_inj; eauto.
+    apply nextinstr_pres_inject. repeat apply undef_regs_pres_inject. auto.
+    eapply storev_pres_glob_block_valid; eauto.
+Qed.
+
+
+Ltac solve_store_load :=
+  match goal with
+  | [ H : Asm.exec_instr _ _ _ _ _ _ = Next _ _ |- _ ] =>
+    unfold Asm.exec_instr in H; simpl in H; solve_store_load
+  | [ H : Asm.exec_store _ _ _ _ _ _ _ _ = Next _ _ |- _ ] =>
+    exploit exec_store_step; eauto
+  | [ H : Asm.exec_load _ _ _ _ _ _ _ = Next _ _ |- _ ] =>
+    exploit exec_load_step; eauto
+  end.
+
+Lemma eval_testcond_inject: forall j c rs1 rs2,
+    regset_inject j rs1 rs2 ->
+    Val.opt_lessdef (Asm.eval_testcond c rs1) (Asm.eval_testcond c rs2).
+Proof.
+  intros. destruct c; simpl; try solve_opt_lessdef.
+Qed.
+
+Hint Resolve nextinstr_nf_pres_inject nextinstr_pres_inject regset_inject_expand
+  regset_inject_expand_vundef_left undef_regs_pres_inject
+  Val.zero_ext_inject Val.sign_ext_inject Val.longofintu_inject Val.longofint_inject
+  Val.singleoffloat_inject Val.loword_inject Val.floatofsingle_inject Val.intoffloat_inject Val.maketotal_inject
+  Val.intoffloat_inject Val.floatofint_inject Val.intofsingle_inject Val.singleofint_inject
+  Val.longoffloat_inject Val.floatoflong_inject Val.longofsingle_inject Val.singleoflong_inject
+  eval_addrmode32_inject eval_addrmode64_inject eval_addrmode_inject
+  Val.neg_inject Val.negl_inject Val.add_inject Val.addl_inject
+  Val.sub_inject Val.subl_inject Val.mul_inject Val.mull_inject Val.mulhs_inject Val.mulhu_inject
+  Val.mullhs_inject Val.mullhu_inject Val.shr_inject Val.shrl_inject Val.or_inject Val.orl_inject
+  Val.xor_inject Val.xorl_inject Val.and_inject Val.andl_inject Val.notl_inject
+  Val.shl_inject Val.shll_inject Val.vzero_inject Val.notint_inject
+  Val.shru_inject Val.shrlu_inject Val.ror_inject Val.rorl_inject
+  compare_ints_inject compare_longs_inject compare_floats_inject compare_floats32_inject
+  Val.addf_inject Val.subf_inject Val.mulf_inject Val.divf_inject Val.negf_inject Val.absf_inject
+  Val.addfs_inject Val.subfs_inject Val.mulfs_inject Val.divfs_inject Val.negfs_inject Val.absfs_inject
+  val_of_optbool_lessdef eval_testcond_inject Val.offset_ptr_inject: inject_db.
+
+Ltac solve_exec_instr :=
+  match goal with
+  | [ |- Next _ _ = Next _ _ ] =>
+    reflexivity
+  | [ |- context [eval_testcond _ _] ]=>
+    unfold eval_testcond; solve_exec_instr
+  | [ H: Asm.eval_testcond ?c ?r = _ |- context [Asm.eval_testcond ?c ?r] ] =>
+    rewrite H; solve_exec_instr
+  | [ H: _ = Asm.eval_testcond ?c ?r |- context [Asm.eval_testcond ?c ?r] ] =>
+    rewrite <- H; solve_exec_instr
+  end.
+
+Ltac solve_match_states :=
+  match goal with
+  | [ H: Asm.Stuck = Next _ _ |- _ ] => inv H
+  | [ |- exists _, _ ] => eexists; solve_match_states
+  | [ |- Next _ _ = Next _ _ /\ match_states _ _ ] =>
+    split; [reflexivity | econstructor; eauto; solve_match_states]
+  | [ |- (exec_instr _ _ _ _ = Next _ _) /\ match_states _ _ ] =>
+    split; [simpl; solve_exec_instr | econstructor; eauto; solve_match_states]
+  | [ |- regset_inject _ _ _ ] =>
+    eauto 10 with inject_db
+  end.
+
+Ltac destr_eval_testcond :=
+  match goal with
+  | [ H : match Asm.eval_testcond ?c ?rs with | _ => _ end = Next _ _ |- _ ] =>
+    let ETEQ := fresh "ETEQ" in (
+      destruct (Asm.eval_testcond c rs) eqn:ETEQ); destr_eval_testcond
+  | [ H : Some ?b = Asm.eval_testcond _ _ |- _ ] =>
+    match b with
+    | true => fail 1
+    | false => fail 1
+    | _ => destruct b; destr_eval_testcond
+    end
+  | [ H : Asm.eval_testcond _ _ = Some ?b |- _] =>
+    match b with
+    | true => fail 1
+    | false => fail 1
+    | _ => destruct b; destr_eval_testcond
+    end
+  | [ H : Asm.Next _ _ = Next _ _ |- _ ] =>
+    inv H; destr_eval_testcond
+  | [ H: Val.opt_lessdef (Some true) (Asm.eval_testcond _ _) |- _ ] =>
+    inv H; destr_eval_testcond
+  | [ H: Val.opt_lessdef (Some false) (Asm.eval_testcond _ _) |- _ ] =>
+    inv H; destr_eval_testcond
+  | _ => idtac
+  end.
+
+Ltac destr_match_outcome :=
+  match goal with
+  | [ H: Asm.Stuck = Next _ _ |- _ ] => inv H
+  | [ H: Asm.Next _ _ = Next _ _ |- _ ] => inv H; destr_match_outcome
+  | [ H: match ?a with _ => _ end = Next _ _ |- _] =>
+    let EQ := fresh "EQ" in (destruct a eqn:EQ; destr_match_outcome)
+  | _ => idtac
+  end.
+
+
+Lemma goto_ofs_pres_mem : forall f l rs1 m1 rs1' m1',
+    Asm.goto_ofs ge f l rs1 m1 = Next rs1' m1' -> m1 = m1'.
+Proof.
+  unfold Asm.goto_label. intros.
+  unfold Asm.goto_ofs in H. 
+  repeat destr_in H.
+Qed.
+
+Lemma goto_ofs_inject : forall rs1 rs2 f l j m1 m2 rs1' m1'
+                            (RINJ: regset_inject j rs1 rs2),
+    Asm.goto_ofs ge f l rs1 m1 = Next rs1' m1' ->
+    exists rs2', goto_ofs f l rs2 m2 = Next rs2' m2 /\
+            regset_inject j rs1' rs2'.
+Proof.
+  intros. unfold Asm.goto_ofs in H.
+  destr_in H. destr_in H. inv H.
+  unfold goto_ofs.
+  generalize (RINJ PC). rewrite Heqv.
+  intros NJ. inv NJ.
+  eexists; split; eauto.
+  apply regset_inject_expand; auto.
+  eapply Val.inject_ptr; eauto.
+  repeat rewrite Ptrofs.add_assoc.
+  f_equal.
+  rewrite Ptrofs.add_commut.
+  repeat rewrite Ptrofs.add_assoc.
+  auto.
+Qed.
+
+Lemma goto_ofs_inject' : forall l f j rs1 rs2 m1 m2 rs1' m1'
+                                (RINJ: regset_inject j rs1 rs2),
+    Asm.goto_ofs ge f l ((rs1 # RAX <- Vundef) # RDX <- Vundef) m1 = Next rs1' m1' ->
+    exists rs2',
+      goto_ofs f l ((rs2 # RAX <- Vundef) # RDX <- Vundef) m2 = Next rs2' m2 /\
+      regset_inject j rs1' rs2'.
+Proof.
+  intros. 
+  eapply goto_ofs_inject; eauto.
+  repeat apply regset_inject_expand; auto.
+Qed.
+
+Lemma extcall_pres_glob_block_valid : forall ef ge vargs m1 t vres m2,
+  external_call ef ge vargs m1 t vres m2 -> glob_block_valid m1 -> glob_block_valid m2.
+Proof.
+  unfold glob_block_valid in *. intros.
+  eapply external_call_valid_block; eauto.
+Qed.
+
+
+(** The internal step preserves the invariant *)
+Lemma exec_instr_step : forall j rs1 rs2 m1 m2 rs1' m1' i ofs f b
+                        (MINJ: Mem.inject j (def_frame_inj m1) m1 m2)
+                        (MATCHSMINJ: match_inj j)
+                        (RSINJ: regset_inject j rs1 rs2)
+                        (GBVALID: glob_block_valid m1),
+    rs1 PC = Vptr b ofs ->
+    Globalenvs.Genv.find_funct_ptr ge b = Some (Internal f) ->
+    Asm.find_instr (Ptrofs.unsigned ofs) (Asm.fn_code f) = Some i ->
+    RealAsm.exec_instr ge f i rs1 m1 = Next rs1' m1' ->
+    exists rs2' m2',
+      exec_instr tge i rs2 m2 = Next rs2' m2' /\
+      match_states (State rs1' m1') (State rs2' m2').
+Proof.
+  intros.
+  destruct i; inv H2; simpl in *; 
+    try first [solve_store_load |
+               solve_match_states].
+
+  - (* Pmov_rs *)
+    apply nextinstr_nf_pres_inject.
+    apply regset_inject_expand; auto.
+    inv MATCHSMINJ.
+    unfold Globalenvs.Genv.symbol_address.
+    destruct (Globalenvs.Genv.find_symbol ge id) eqn:FINDSYM; auto.
+    exploit agree_inj_globs0; eauto.
+    intros (b1 & ofs1 & GLBL & JB).
+    erewrite Genv.find_sym_to_addr with (ofs:=ofs1); eauto.
+    rewrite <- (Ptrofs.add_zero_l ofs1).
+    eapply Val.inject_ptr; eauto.
+    rewrite Ptrofs.repr_unsigned. auto.
+
+  (* Divisions *)
+  - destr_match_outcome. 
+    generalize (RSINJ Asm.RDX). generalize (RSINJ Asm.RAX). generalize (RSINJ r1).
+    rewrite EQ, EQ0, EQ1. inversion 1; subst. inversion 1; subst. inversion 1; subst.
+    eexists; eexists. split. simpl. rewrite EQ2. auto.
+    eapply match_states_intro; eauto with inject_db.
+
+  - destr_match_outcome. 
+    generalize (RSINJ Asm.RDX). generalize (RSINJ Asm.RAX). generalize (RSINJ r1).
+    rewrite EQ, EQ0, EQ1. inversion 1; subst. inversion 1; subst. inversion 1; subst.
+    eexists; eexists. split. simpl. rewrite EQ2. auto.
+    eapply match_states_intro; eauto with inject_db.
+
+  - destr_match_outcome. 
+    generalize (RSINJ Asm.RDX). generalize (RSINJ Asm.RAX). generalize (RSINJ r1).
+    rewrite EQ, EQ0, EQ1. inversion 1; subst. inversion 1; subst. inversion 1; subst.
+    eexists; eexists. split. simpl. rewrite EQ2. auto.
+    eapply match_states_intro; eauto with inject_db.
+
+  - destr_match_outcome. 
+    generalize (RSINJ Asm.RDX). generalize (RSINJ Asm.RAX). generalize (RSINJ r1).
+    rewrite EQ, EQ0, EQ1. inversion 1; subst. inversion 1; subst. inversion 1; subst.
+    eexists; eexists. split. simpl. rewrite EQ2. auto.
+    eapply match_states_intro; eauto with inject_db.
+     
+  - (* Pcmov *)
+    exploit (eval_testcond_inject j c rs1 rs2); eauto.
+    intros. 
+    destr_eval_testcond; try solve_match_states.
+    destruct (Asm.eval_testcond c rs2) eqn:EQ'. destruct b0; solve_match_states.
+    solve_match_states.
+
+  - (* Pjmp_l *)
+    assert (instr_valid (Pjmp_l l)) as NJ.
+    { eapply instr_is_valid; eauto. }
+    red in NJ. cbn in NJ. contradiction.
+
+  - (* Pjmp *)
+    repeat destr_in H4.
+    destruct ros; simpl in *.
+    + do 2 eexists; split; eauto.
+      econstructor; eauto.
+      apply regset_inject_expand; auto.
+    + do 2 eexists; split; eauto.
+      econstructor; eauto.
+      apply regset_inject_expand; auto.
+      inversion MATCHSMINJ.
+      unfold Globalenvs.Genv.symbol_address. destr_match; auto.
+      exploit (agree_inj_globs0 i b0); eauto.
+      intros (b1 & ofs1 & LBLOFS & JB).
+      erewrite Genv.find_sym_to_addr with (ofs:=ofs1); eauto.
+      rewrite <- (Ptrofs.add_zero_l ofs1).
+      eapply Val.inject_ptr; eauto.
+      rewrite Ptrofs.repr_unsigned. auto.
+
+  - (* Pjcc *)
+    assert (instr_valid (Pjcc c l)) as NJ.
+    { eapply instr_is_valid; eauto. }
+    red in NJ. cbn in NJ. contradiction.
+    
+  - (* Pjcc2 *)
+    assert (instr_valid (Pjcc2 c1 c2 l)) as NJ.
+    { eapply instr_is_valid; eauto. }
+    red in NJ. cbn in NJ. contradiction.
+
+  - (* Pjmptbl *)
+    admit.
+(***** Remove Proofs By Chris Start ******)
+(*      
+    assert (instr_valid (Pjmptbl r tbl)) as NJ.
+    { eapply instr_is_valid; eauto. }
+    red in NJ. cbn in NJ. contradiction.
+*)
+(***** Remove Proofs By Chris End ******)
+  - (* Pcall *)    
+    repeat destr_in H4.
+    generalize (RSINJ PC).
+    edestruct storev_mapped_inject' as (m2' & ST & MINJ'). apply MINJ. eauto.
+    apply Val.offset_ptr_inject. eauto.
+    apply Val.offset_ptr_inject. eauto.
+    do 2 eexists; split; eauto. simpl.
+    rewrite ST. eauto.
+    econstructor; eauto.
+    repeat apply regset_inject_expand; auto.
+    apply Val.offset_ptr_inject. eauto.
+    destruct ros; simpl; repeat apply regset_inject_expand; auto.
+    exploit (inject_symbol_address j i Ptrofs.zero); eauto.
+    apply Val.offset_ptr_inject. eauto.
+    eapply storev_pres_glob_block_valid; eauto. 
+ 
+  - (* Pret *)
+    repeat destr_in H4. simpl.
+    exploit Mem.loadv_inject; eauto. intros (v2 & LD & VI). rewrite LD.
+    eexists _, _; split; eauto. econstructor; eauto.
+    repeat apply regset_inject_expand; auto.
+    apply Val.offset_ptr_inject. eauto.
+
+  - (* Pallocframe *)
+    assert (instr_valid (Pallocframe sz ofs_ra)) as NJ.
+    { eapply instr_is_valid; eauto. }
+    red in NJ. cbn in NJ. contradiction.
+
+  - (* Pfreeframe *)
+    assert (instr_valid (Pfreeframe sz ofs_ra)) as NJ.
+    { eapply instr_is_valid; eauto. }
+    red in NJ. cbn in NJ. contradiction.
+
+  - (* Pload_parent_pointer *)
+    assert (instr_valid (Pload_parent_pointer rd sz)) as NJ.
+    { eapply instr_is_valid; eauto. }
+    red in NJ. cbn in NJ. contradiction.
+    
+  - (* Pjmp_l_rel *)
+    unfold Asm.goto_ofs in H4. 
+    destruct (rs1 Asm.PC) eqn:PC1; inv H4. 
+    destruct (Globalenvs.Genv.find_funct_ptr ge b0); inv H3.
+    generalize (RSINJ PC). rewrite PC1.
+    intros INJ. inv INJ. eauto.
+    eexists; eexists. split. 
+    unfold goto_ofs. 
+    rewrite <- H4. eauto.
+    eapply match_states_intro; eauto.
+    apply regset_inject_expand; auto. 
+    rewrite H in *. inv PC1. inv H.
+    eapply Val.inject_ptr; eauto. 
+    repeat rewrite Ptrofs.add_assoc. f_equal.
+    match goal with
+    | [ |- _ = Ptrofs.add _ (Ptrofs.add ?b ?c) ] =>
+      rewrite (Ptrofs.add_commut b c)
+    end.
+    match goal with
+    | [ |- _ = Ptrofs.add ?a ?b ] =>
+      rewrite (Ptrofs.add_commut a b)
+    end.
+    repeat rewrite Ptrofs.add_assoc. f_equal.
+    apply Ptrofs.add_commut.
+    
+  - (* Pjcc_rel *)
+    exploit (eval_testcond_inject j c rs1 rs2); eauto.
+    intros.
+    destr_eval_testcond; try solve_match_states.
+    exploit goto_ofs_pres_mem; eauto. intros. subst.
+    generalize (goto_ofs_inject _ _ _ _ _ m1' m2 _ _ RSINJ H4).
+    intros (rs2' & GOTO & RINJ').
+    exists rs2', m2. split; auto.
+    eapply match_states_intro; eauto.
+
+  - (* Pjcc2_rel *)
+    exploit (eval_testcond_inject j c1 rs1 rs2); eauto.
+    exploit (eval_testcond_inject j c2 rs1 rs2); eauto.
+    intros ELF1 ELF2.
+    destr_eval_testcond; try solve_match_states.
+    exploit goto_ofs_pres_mem; eauto. intros. subst.
+    generalize (goto_ofs_inject _ _ _ _ _ m1' m2 _ _ RSINJ H4).
+    intros (rs2' & GOTO & RINJ').
+    exists rs2', m2. split; auto.
+    eapply match_states_intro; eauto.
+
+  - (* Pjmptbl_rel *)
+    admit.
+(***** Remove Proofs By Chris Start ******)
+(*      
+    destruct (rs1 r) eqn:REQ; inv H4.
+    destruct (list_nth_z tbl (Int.unsigned i)) eqn:LEQ; inv H3.
+    assert (rs2 r = Vint i) by
+        (generalize (RSINJ r); rewrite REQ; inversion 1; auto).
+    exploit goto_ofs_pres_mem; eauto. intros. subst.
+    generalize (goto_ofs_inject' _ _ _ _ _ m1' m2 _ _ RSINJ H4).
+    intros (rs2' & GLBL & RSINJ').
+    exists rs2', m2. rewrite H2. rewrite LEQ.
+    split; auto.
+    eapply match_states_intro; eauto.
+*)
+(***** Remove Proofs By Chris End ******)
+Admitted.
+
+
+Theorem step_simulation:
+  forall S1 t S2,
+    RealAsm.step ge S1 t S2 ->
+    forall S1' (MS: match_states S1 S1'),
+    exists S2',
+      step tge S1' t S2' /\
+      match_states S2 S2'.
+Proof.
+  destruct 1; intros; inv MS.
+
+  - (* Internal step *)
+    unfold regset_inject in RSINJ. generalize (RSINJ Asm.PC). rewrite H. 
+    inversion 1; subst.
+    exploit (agree_inj_instrs j MATCHINJ b b2 f ofs delta i); eauto.
+    intros FIND.
+    exploit (exec_instr_step j rs rs'0 m m'0 rs' m' i); eauto.
+    intros (rs2' & m2' & FEXEC & MS1).
+    exists (State rs2' m2'). split; auto.
+    eapply exec_step_internal; eauto.
+    eapply (agree_inj_int_funct j MATCHINJ); eauto.
+        
+  - (* Builtin *)
+    unfold regset_inject in RSINJ. generalize (RSINJ Asm.PC). rewrite H.
+    inversion 1; subst.
+    exploit (agree_inj_instrs j MATCHINJ b b2 f ofs delta (Asm.Pbuiltin ef args res)); auto.
+    intros FIND.
+    exploit (eval_builtin_args_inject j m m'0 rs rs'0 (rs Asm.RSP) (rs'0 Asm.RSP) args vargs); auto.
+    intros (vargs' & EBARGS & ARGSINJ).
+    assert (Globalenvs.Genv.to_senv ge = (Genv.genv_senv tge)) as SENVEQ. 
+    { eapply transf_prog_pres_senv; eauto. }
+    generalize (external_call_inject ge j vargs vargs' m m'0 m' vres t ef ARGSINJ MINJ H3).
+    rewrite SENVEQ.
+    intros (j' & vres2 & m2' & EXTCALL & RESINJ & MINJ' & INJINCR & INJSEP).
+    set (rs' := nextinstr_nf (set_res res vres2 (undef_regs (map preg_of (Machregs.destroyed_by_builtin ef)) rs'0)) 
+                             (Ptrofs.repr (instr_size (Pbuiltin ef args res)))).
+    exploit (fun b ofs => exec_step_builtin tge b ofs
+                                         ef args res rs'0  m'0 vargs' t vres2 rs' m2'); eauto. 
+    eapply (agree_inj_int_funct j MATCHINJ); eauto.
+    intros FSTEP. eexists; split; eauto.
+    eapply match_states_intro with (j:=j'); eauto.
+    (* Supposely the following propreties can proved by separation property of injections *)
+    + eapply (inject_pres_match_sminj j); eauto.
+    + subst rs'. intros. 
+      assert (regset_inject j' rs rs'0) by 
+          (eapply regset_inject_incr; eauto).
+      set (dregs := (map Asm.preg_of (Machregs.destroyed_by_builtin ef))) in *.
+      generalize (undef_regs_pres_inject j' rs rs'0 dregs H5). intros.
+      set (rs1 := (Asm.undef_regs dregs rs)) in *.
+      set (rs2 := (Asm.undef_regs dregs rs'0)) in *.
+      generalize (fun h => set_res_pres_inject res j' 
+                  rs1 rs2 h vres vres2 RESINJ).
+      set (rs3 := (Asm.set_res res vres rs1)) in *.
+      set (rs4 := (Asm.set_res res vres2 rs2)) in *.
+      intros.
+      eauto with inject_db.
+    + eapply extcall_pres_glob_block_valid; eauto.
+
+  - (* External call *)
+    unfold regset_inject in RSINJ. generalize (RSINJ Asm.PC). rewrite H. 
+    inversion 1; subst. rewrite Ptrofs.add_zero_l in H6.
+    exploit Mem.loadv_inject. apply MINJ. apply LOADRA. eauto. intros (v2 & LRA & VI).
+    edestruct (extcall_arguments_inject) as (args2 & ARGSINJ & EXTCALLARGS); eauto.
+    apply regset_inject_expand. eauto.
+    apply Val.offset_ptr_inject. eauto.
+    assert (Globalenvs.Genv.to_senv ge = (Genv.genv_senv tge)) as SENVEQ. 
+    { eapply transf_prog_pres_senv; eauto. }
+    exploit (external_call_inject ge j args args2 ); eauto.
+    rewrite SENVEQ.
+    
+    intros (j' & res' & m2'' & EXTCALL & RESINJ & MINJ' & INJINCR & INJSEP).
+    exploit (fun ofs => exec_step_external tge b2 ofs ef args2 res'); eauto.
+    eapply agree_inj_ext_funct; eauto.
+    + intro; subst. inv VI. congruence.
+    + intros FSTEP. eexists. split. apply FSTEP.
+      eapply match_states_intro with (j := j'); eauto.
+      * eapply (inject_pres_match_sminj j); eauto.
+      * assert (regset_inject j' rs rs'0) by 
+            (eapply regset_inject_incr; eauto).
+        set (dregs := (map Asm.preg_of Conventions1.destroyed_at_call)) in *.
+        generalize (undef_regs_pres_inject j' rs rs'0 dregs H4). intros.
+        set (rs1 := (Asm.undef_regs dregs rs)) in *.
+        set (rs2 := (Asm.undef_regs dregs rs'0)) in *.
+        set (cdregs := (CR Asm.ZF :: CR Asm.CF :: CR Asm.PF :: CR Asm.SF :: CR Asm.OF :: nil)) in *.
+        generalize (undef_regs_pres_inject j' rs1 rs2 cdregs). intros.
+        set (rs3 := (Asm.undef_regs cdregs rs1)) in *.
+        set (rs4 := (Asm.undef_regs cdregs rs2)) in *.
+        generalize (set_pair_pres_inject j' rs3 rs4 res res' 
+                                         (Asm.loc_external_result (ef_sig ef))).
+        intros.
+        apply regset_inject_expand; auto.
+        apply regset_inject_expand; auto.
+        apply regset_inject_expand; auto. eapply val_inject_incr; eauto.
+        apply Val.offset_ptr_inject; eauto.
+      * eapply extcall_pres_glob_block_valid; eauto.
+Qed.
+
+
+(** ** Matching of the Final States*)
+Lemma transf_final_states:
+  forall st1 st2 r,
+  match_states st1 st2 -> Asm.final_state st1 r -> final_state st2 r.
+Proof.
+  intros st1 st2 r MATCH FINAL.
+  inv FINAL. inv MATCH. constructor. 
+  - red in RSINJ. generalize (RSINJ PC). rewrite H. 
+    unfold Vnullptr. destruct Archi.ptr64; inversion 1; auto.
+  - red in RSINJ. generalize (RSINJ RAX). rewrite H0.
+    inversion 1. auto.
+Qed.
+
+(** ** The Main Correctness Theorem *)
+Lemma transf_program_correct:
+  forward_simulation (RealAsm.semantics prog (Pregmap.init Vundef)) 
+                     (semantics tprog (Pregmap.init Vundef)).
+Proof.
+  intros. apply forward_simulation_step with match_states.
+  - simpl. intros. 
+    unfold match_prog in TRANSF. unfold transf_program in TRANSF.
+    repeat destr_in TRANSF. cbn.
+    rewrite add_external_globals_pres_senv. cbn. auto.
+  - simpl. intros s1 IS. 
+    exploit transf_initial_states; eauto.
+    intros.
+    rewrite Pregmap.gi. auto.
+  - simpl. intros s1 s2 r MS FS. eapply transf_final_states; eauto.
+  - simpl. intros s1 t s1' STEP s2 MS. 
+    edestruct step_simulation as (STEP' & MS'); eauto.
+Qed.
+
+
+End PRESERVATION.
